src/core-props/bir_program_multistep_propsScript.sml
@@ -4,7 +4,8 @@ open bir_auxiliaryTheory bir_immTheory bir_valuesTheory;
 open bir_imm_expTheory bir_mem_expTheory bir_envTheory;
 open bir_expTheory bir_programTheory;
 open bir_program_valid_stateTheory;
-open llistTheory wordsLib;
+open llistTheory wordsLib pred_setTheory;
+open HolBACoreSimps
 
 val _ = new_theory "bir_program_multistep_props";
 
@@ -13,7 +14,6 @@ val _ = new_theory "bir_program_multistep_props";
    reasoning with directly. In this theory, some basic properties and rewrite
    rules are derived for them.                                               *)
 (* ------------------------------------------------------------------------- *)
-
 
 
 (***************************)
@@ -79,32 +79,526 @@ Induct_on `n` >> REWRITE_TAC[bir_exec_infinite_steps_fun_REWRS2] >>
 ASM_SIMP_TAC std_ss [bir_exec_step_valid_pc]);
 
 
+(*****************************************)
+(* bir_exec_infinite_steps_fun_COUNT_PCs *)
+(*****************************************)
+
+val bir_exec_infinite_steps_fun_COUNT_PCs_END_DEF = store_thm ("bir_exec_infinite_steps_fun_COUNT_PCs_END_DEF",
+ ``(!pc_cond p st.
+      bir_exec_infinite_steps_fun_COUNT_PCs pc_cond p st 0 = 0) /\
+   (!pc_cond p st n.
+     bir_exec_infinite_steps_fun_COUNT_PCs pc_cond p st (SUC n) =
+     (let r =
+            bir_exec_infinite_steps_fun_COUNT_PCs pc_cond p
+              st n
+      in
+        if bir_state_COUNT_PC pc_cond (bir_exec_infinite_steps_fun p st (SUC n)) then SUC r
+        else r))``,
+
+CONJ_TAC >- REWRITE_TAC[bir_exec_infinite_steps_fun_COUNT_PCs_def] >>
+GEN_TAC >> GEN_TAC >> Induct_on `n` >- (
+  SIMP_TAC std_ss [bir_exec_infinite_steps_fun_COUNT_PCs_def, LET_DEF,
+    bir_exec_infinite_steps_fun_REWRS]
+) >>
+ONCE_REWRITE_TAC[bir_exec_infinite_steps_fun_COUNT_PCs_def, bir_programTheory.bir_exec_infinite_steps_fun_REWRS] >>
+ASM_SIMP_TAC std_ss [LET_DEF] >>
+METIS_TAC[]);
+
+
+val bir_exec_infinite_steps_fun_COUNT_PCs_ADD = store_thm (
+"bir_exec_infinite_steps_fun_COUNT_PCs_ADD",
+ ``!pc_cond p st n1 n2.
+      bir_exec_infinite_steps_fun_COUNT_PCs pc_cond p st (n1 + n2) =
+      (bir_exec_infinite_steps_fun_COUNT_PCs pc_cond p st n1 +
+       bir_exec_infinite_steps_fun_COUNT_PCs pc_cond p (bir_exec_infinite_steps_fun p st n1) n2)``,
+
+Induct_on `n2` >> (
+  ASM_SIMP_TAC (std_ss++boolSimps.LIFT_COND_ss) [bir_exec_infinite_steps_fun_COUNT_PCs_END_DEF,
+    arithmeticTheory.ADD_CLAUSES, LET_DEF,
+    bir_exec_infinite_steps_fun_ADD]
+));
+
+
+val bir_exec_infinite_steps_fun_PC_COND_SET_def = Define
+  `bir_exec_infinite_steps_fun_PC_COND_SET pc_cond p state =
+   {i | i <> 0 /\ bir_state_COUNT_PC pc_cond (bir_exec_infinite_steps_fun p state i)}`;
+
+val IN_bir_exec_infinite_steps_fun_PC_COND_SET = store_thm (
+  "IN_bir_exec_infinite_steps_fun_PC_COND_SET",
+
+``!i pc_cond p st. i IN (bir_exec_infinite_steps_fun_PC_COND_SET pc_cond p st) <=>
+   (i <> 0) /\ (bir_state_COUNT_PC pc_cond (bir_exec_infinite_steps_fun p st i))``,
+
+SIMP_TAC (std_ss) [bir_exec_infinite_steps_fun_PC_COND_SET_def,
+  GSPECIFICATION]);
+
+
+val INTER_INSERT_aux = prove (``(s1 INTER (e INSERT s2)) =
+  if (e IN s1) then e INSERT (s1 INTER s2) else (s1 INTER s2)``,
+SIMP_TAC (std_ss++boolSimps.LIFT_COND_ss++boolSimps.EQUIV_EXTRACT_ss) [EXTENSION,
+  IN_INTER, IN_INSERT] >>
+METIS_TAC[]);
+
+
+val bir_exec_infinite_steps_fun_COUNT_PCs_ALT_DEF = store_thm (
+ "bir_exec_infinite_steps_fun_COUNT_PCs_ALT_DEF",
+``!pc_cond p i state. bir_exec_infinite_steps_fun_COUNT_PCs pc_cond p state i =
+  CARD ((bir_exec_infinite_steps_fun_PC_COND_SET pc_cond p state) INTER
+        (count (SUC i)))``,
+
+GEN_TAC >> GEN_TAC >>
+Induct >- (
+  REWRITE_TAC[COUNT_SUC, INTER_INSERT_aux] >>
+  SIMP_TAC std_ss [INTER_EMPTY,
+    CARD_EMPTY, bir_exec_infinite_steps_fun_COUNT_PCs_def, COUNT_ZERO,
+      IN_bir_exec_infinite_steps_fun_PC_COND_SET]
+) >>
+GEN_TAC >>
+ONCE_REWRITE_TAC[COUNT_SUC] >>
+ASM_SIMP_TAC arith_ss [bir_exec_infinite_steps_fun_COUNT_PCs_END_DEF, LET_DEF,
+  INTER_INSERT_aux, IN_bir_exec_infinite_steps_fun_PC_COND_SET] >>
+CASE_TAC >>
+SIMP_TAC std_ss [CARD_INSERT, FINITE_INTER, FINITE_COUNT,
+  IN_INTER, IN_COUNT]);
+
+
+val bir_state_COUNT_PC_MONO = store_thm (
+ "bir_state_COUNT_PC_MONO",
+``!pc_cond pc_cond'.
+   (!pc. pc_cond pc ==> pc_cond' pc) ==>
+   (!st. bir_state_COUNT_PC pc_cond st ==> bir_state_COUNT_PC pc_cond' st)``,
+
+NTAC 2 GEN_TAC >>
+STRIP_TAC >> GEN_TAC >>
+SIMP_TAC std_ss [bir_state_COUNT_PC_def] >>
+Cases_on `st.bst_status` >> (
+  ASM_SIMP_TAC (std_ss++bir_TYPES_ss) []
+));
+
+
+val bir_exec_infinite_steps_fun_COUNT_PCs_MONO_PC_COND = store_thm (
+"bir_exec_infinite_steps_fun_COUNT_PCs_MONO_PC_COND",
+``!pc_cond pc_cond' p state i.
+   (!pc. pc_cond pc ==> pc_cond' pc) ==>
+   bir_exec_infinite_steps_fun_COUNT_PCs pc_cond p state i <=
+   bir_exec_infinite_steps_fun_COUNT_PCs pc_cond' p state i``,
+
+REPEAT STRIP_TAC >>
+Induct_on `i` >- (
+  SIMP_TAC std_ss [bir_exec_infinite_steps_fun_COUNT_PCs_def]
+) >>
+ASM_SIMP_TAC std_ss [bir_exec_infinite_steps_fun_COUNT_PCs_END_DEF, LET_DEF] >>
+Q.ABBREV_TAC `st' = (bir_exec_infinite_steps_fun p state (SUC i))` >>
+Cases_on `bir_state_COUNT_PC pc_cond st'` >- (
+  `bir_state_COUNT_PC pc_cond' st'` by METIS_TAC[bir_state_COUNT_PC_MONO] >>
+  ASM_SIMP_TAC std_ss []
+) >>
+ASM_SIMP_TAC (arith_ss++boolSimps.LIFT_COND_ss) []);
+
+
+val bir_exec_infinite_steps_fun_COUNT_PCs_LESS_EQ = store_thm (
+"bir_exec_infinite_steps_fun_COUNT_PCs_LESS_EQ",
+``!pc_cond p state i.
+   bir_exec_infinite_steps_fun_COUNT_PCs pc_cond p state i <= i``,
+
+GEN_TAC >> GEN_TAC >>
+Induct_on `i` >> (
+  ASM_SIMP_TAC (arith_ss++boolSimps.LIFT_COND_ss) [bir_exec_infinite_steps_fun_COUNT_PCs_def, LET_DEF]
+) >>
+METIS_TAC[arithmeticTheory.LESS_EQ_SUC_REFL, arithmeticTheory.LESS_EQ_TRANS]);
+
+
+val bir_exec_infinite_steps_fun_COUNT_PCs_EQ = store_thm (
+"bir_exec_infinite_steps_fun_COUNT_PCs_EQ",
+``!pc_cond p state i.
+
+   (bir_exec_infinite_steps_fun_COUNT_PCs pc_cond p state i = i) <=> (
+   !j. j < i ==> bir_state_COUNT_PC pc_cond (bir_exec_infinite_steps_fun p state (SUC j)))``,
+
+GEN_TAC >> GEN_TAC >>
+Induct_on `i` >> (
+  ASM_SIMP_TAC (arith_ss++boolSimps.LIFT_COND_ss) [
+    bir_exec_infinite_steps_fun_COUNT_PCs_END_DEF, LET_DEF, prim_recTheory.LESS_THM,
+    DISJ_IMP_THM, FORALL_AND_THM]
+) >>
+GEN_TAC >>
+DISJ2_TAC >>
+`~(SUC i <= i)` by DECIDE_TAC >>
+METIS_TAC[bir_exec_infinite_steps_fun_COUNT_PCs_LESS_EQ]);
+
+
+val bir_state_COUNT_PC_ALL_STEPS = store_thm ("bir_state_COUNT_PC_ALL_STEPS",
+  ``!st. bir_state_COUNT_PC (\_. T) st``,
+
+GEN_TAC >>
+Cases_on `st.bst_status` >> (
+  ASM_SIMP_TAC (std_ss++bir_TYPES_ss) [bir_state_COUNT_PC_def]
+));
+
+
+val bir_exec_infinite_steps_fun_COUNT_PCs_EQ_COUNT_ALL_STEPS = store_thm (
+"bir_exec_infinite_steps_fun_COUNT_PCs_EQ_COUNT_ALL_STEPS",
+``!p state i.
+   (bir_exec_infinite_steps_fun_COUNT_PCs (\_. T) p state i = i)``,
+SIMP_TAC std_ss [bir_exec_infinite_steps_fun_COUNT_PCs_EQ,
+  bir_state_COUNT_PC_ALL_STEPS]);
+
+
+val bir_exec_infinite_steps_fun_COUNT_PCs_MONO = store_thm ("bir_exec_infinite_steps_fun_COUNT_PCs_MONO",
+
+``!pc_cond p state i j.
+   i <= j ==>
+   bir_exec_infinite_steps_fun_COUNT_PCs pc_cond p state i <=
+   bir_exec_infinite_steps_fun_COUNT_PCs pc_cond p state j``,
+
+SIMP_TAC std_ss [bir_exec_infinite_steps_fun_COUNT_PCs_ALT_DEF] >>
+REPEAT STRIP_TAC >>
+IRULE_TAC CARD_SUBSET >- (
+  SIMP_TAC std_ss [FINITE_INTER, FINITE_COUNT]
+) >>
+ASM_SIMP_TAC arith_ss [SUBSET_DEF, IN_INTER, IN_COUNT]);
+
+
+
+val bir_exec_infinite_steps_fun_COUNT_PCs_COMPLETE = store_thm (
+"bir_exec_infinite_steps_fun_COUNT_PCs_COMPLETE",
+``!pc_cond p state i c_j.
+   (c_j < bir_exec_infinite_steps_fun_COUNT_PCs pc_cond p state i) ==>
+   (?j. j < i /\ (bir_exec_infinite_steps_fun_COUNT_PCs pc_cond p state j = c_j))``,
+
+REPEAT GEN_TAC >>
+Induct_on `i` >- (
+  SIMP_TAC std_ss [bir_exec_infinite_steps_fun_COUNT_PCs_def]
+) >>
+ASM_SIMP_TAC std_ss [bir_exec_infinite_steps_fun_COUNT_PCs_END_DEF, LET_DEF] >>
+STRIP_TAC >>
+Cases_on `c_j < bir_exec_infinite_steps_fun_COUNT_PCs pc_cond p state i` >- (
+  FULL_SIMP_TAC std_ss [] >>
+  Q.EXISTS_TAC `j` >>
+  ASM_SIMP_TAC arith_ss []
+) >>
+FULL_SIMP_TAC (std_ss++boolSimps.LIFT_COND_ss) [] >>
+Q.EXISTS_TAC `i` >>
+ASM_SIMP_TAC arith_ss []);
+
+
+val bir_exec_infinite_steps_fun_COUNT_PCs_COMPLETE_LESS_EQ = store_thm (
+"bir_exec_infinite_steps_fun_COUNT_PCs_COMPLETE_LESS_EQ",
+``!pc_cond p state i c_j.
+   (c_j <= bir_exec_infinite_steps_fun_COUNT_PCs pc_cond p state i) ==>
+   (?j. j <= i /\ (bir_exec_infinite_steps_fun_COUNT_PCs pc_cond p state j = c_j))``,
+
+METIS_TAC[arithmeticTheory.LESS_OR_EQ,
+  bir_exec_infinite_steps_fun_COUNT_PCs_COMPLETE]);
+
+
+val bir_exec_infinite_steps_fun_COUNT_PCs_COMPLETE_FORALL_NEQ = store_thm (
+ "bir_exec_infinite_steps_fun_COUNT_PCs_COMPLETE_FORALL_NEQ",
+``(!i. (bir_exec_infinite_steps_fun_COUNT_PCs pc_cond p st i <> n)) <=>
+  (!i. (bir_exec_infinite_steps_fun_COUNT_PCs pc_cond p st i < n))``,
+
+Tactical.REVERSE EQ_TAC >- (
+  REPEAT STRIP_TAC >>
+  Q.PAT_X_ASSUM `!i. _` (MP_TAC o Q.SPEC `i`) >>
+  ASM_SIMP_TAC std_ss []
+) >- (
+  REPEAT STRIP_TAC >>
+  CCONTR_TAC >>
+  METIS_TAC[arithmeticTheory.NOT_LESS, bir_exec_infinite_steps_fun_COUNT_PCs_COMPLETE_LESS_EQ]
+));
+
+
+val FINITE_bir_exec_infinite_steps_fun_PC_COND_SET = store_thm (
+"FINITE_bir_exec_infinite_steps_fun_PC_COND_SET",
+``!pc_cond p st c.
+  (FINITE (bir_exec_infinite_steps_fun_PC_COND_SET pc_cond p st) /\
+   CARD (bir_exec_infinite_steps_fun_PC_COND_SET pc_cond p st) < c) <=>
+  (!i. bir_exec_infinite_steps_fun_COUNT_PCs pc_cond p st i < c)``,
+
+REPEAT STRIP_TAC >>
+Q.ABBREV_TAC `CS = bir_exec_infinite_steps_fun_PC_COND_SET pc_cond p st` >>
+EQ_TAC >| [
+  FULL_SIMP_TAC std_ss [bir_exec_infinite_steps_fun_COUNT_PCs_ALT_DEF] >>
+  REPEAT STRIP_TAC >>
+  `CARD (CS INTER (count (SUC i))) <= CARD CS` by
+    METIS_TAC[CARD_SUBSET, INTER_SUBSET] >>
+  DECIDE_TAC,
+
+  STRIP_TAC >>
+  CCONTR_TAC >>
+  `?s. FINITE s /\ (c <= CARD s) /\ s SUBSET CS` by (
+     Cases_on `FINITE CS` >| [
+       Q.EXISTS_TAC `CS` >>
+       FULL_SIMP_TAC arith_ss [SUBSET_REFL],
+
+       METIS_TAC[INFINITE_SUBSET_WITH_CARD_EXISTS, arithmeticTheory.LESS_EQ_REFL]
+     ]
+  ) >>
+  Q.PAT_X_ASSUM `~(_ /\ _)` (K ALL_TAC) >>
+
+  `?i. c <= bir_exec_infinite_steps_fun_COUNT_PCs pc_cond p st i` suffices_by
+     METIS_TAC[bir_exec_infinite_steps_fun_COUNT_PCs_COMPLETE_LESS_EQ,
+       arithmeticTheory.NOT_LESS] >>
+  ASM_SIMP_TAC std_ss [bir_exec_infinite_steps_fun_COUNT_PCs_ALT_DEF] >>
+  Q.EXISTS_TAC `MAX_SET s` >>
+  `s SUBSET (CS INTER count (SUC (MAX_SET s)))` suffices_by
+      METIS_TAC[CARD_SUBSET, FINITE_INTER, FINITE_COUNT, arithmeticTheory.LESS_EQ_TRANS] >>
+  FULL_SIMP_TAC arith_ss [SUBSET_DEF, IN_INTER, IN_COUNT, in_max_set,
+     GSYM arithmeticTheory.LESS_EQ_IFF_LESS_SUC]
+]);
+
+
+val INFINITE_bir_exec_infinite_steps_fun_PC_COND_SET = store_thm (
+"INFINITE_bir_exec_infinite_steps_fun_PC_COND_SET",
+``!pc_cond p st.
+  INFINITE (bir_exec_infinite_steps_fun_PC_COND_SET pc_cond p st) <=>
+  (!c_i. ?i. bir_exec_infinite_steps_fun_COUNT_PCs pc_cond p st i = c_i)``,
+
+METIS_TAC[FINITE_bir_exec_infinite_steps_fun_PC_COND_SET, prim_recTheory.LESS_SUC_REFL,
+   bir_exec_infinite_steps_fun_COUNT_PCs_COMPLETE_FORALL_NEQ]);
+
+
+
+(* If we do not terminate, for most used pc_conds the PC_COND_SET is actually infinite.
+   The most important special case is that we count every beginning of blocks. Since
+   all blocks are finite, we can only loop, if we execute infinitely many blocks. *)
+
+val bir_exec_infinite_steps_fun_block_starts_at_front = store_thm (
+  "bir_exec_infinite_steps_fun_block_starts_at_front",
+``!p st n st_n i.
+     (st_n = bir_exec_infinite_steps_fun p st n) ==>
+     ((bir_exec_infinite_steps_fun p st n).bst_pc.bpc_index = i) ==>
+     ~(bir_state_is_terminated st_n) ==>
+     (i <= n) ==>
+
+     ((bir_exec_infinite_steps_fun p st (n-i)).bst_pc =
+      (st_n.bst_pc with bpc_index := 0))``,
+
+GEN_TAC >> GEN_TAC >>
+Induct_on `i` >- (
+  SIMP_TAC (std_ss++bir_TYPES_ss) [bir_programTheory.bir_programcounter_t_component_equality]
+) >>
+
+FULL_SIMP_TAC std_ss [] >>
+REPEAT STRIP_TAC >>
+Cases_on `n` >> FULL_SIMP_TAC std_ss [] >>
+rename1 `i <= n'` >>
+Q.ABBREV_TAC `st_n' = (bir_exec_infinite_steps_fun p st n')` >>
+Q.PAT_X_ASSUM `!n'. _` (MP_TAC o Q.SPEC `n'`) >>
+FULL_SIMP_TAC std_ss [bir_exec_infinite_steps_fun_REWRS2] >>
+
+Cases_on `bir_state_is_terminated st_n'` >- (
+  FULL_SIMP_TAC std_ss [bir_exec_step_state_def, bir_exec_step_def]
+) >>
+
+Tactical.REVERSE (Cases_on `bir_is_valid_pc p st_n'.bst_pc`) >- (
+  FULL_SIMP_TAC (std_ss++bir_TYPES_ss) [bir_exec_step_state_def, bir_exec_step_def,
+    GSYM bir_get_current_statement_IS_SOME, bir_state_set_failed_def,
+    bir_state_is_terminated_def]
+) >>
+MP_TAC (Q.SPECL [`p`, `st_n'`] bir_exec_step_state_valid_THM) >>
+ASM_SIMP_TAC std_ss [] >>
+STRIP_TAC >>
+Tactical.REVERSE (Cases_on `stmt`) >- (
+  FULL_SIMP_TAC arith_ss [bir_exec_stmt_state_REWRS, bir_exec_stmtE_block_pc]
+) >>
+
+FULL_SIMP_TAC std_ss [bir_exec_stmt_state_REWRS, LET_DEF] >>
+Cases_on `bir_state_is_terminated (bir_exec_stmtB_state b st_n')` >> (
+  FULL_SIMP_TAC std_ss []
+) >>
+FULL_SIMP_TAC (std_ss++bir_TYPES_ss) [bir_pc_next_def,
+  bir_exec_stmtB_pc_unchanged]);
+
+
+
+val bir_is_valid_pc_FINITE = store_thm ("bir_is_valid_pc_FINITE",
+``!p. FINITE {pc | bir_is_valid_pc p pc}``,
+
+Cases >> rename1 `BirProgram p` >>
+Q.ABBREV_TAC `pcs_of_block = \bl. IMAGE (\i. <| bpc_label := bl.bb_label; bpc_index := i |>)
+    (count (SUC (LENGTH bl.bb_statements)))` >>
+
+`{pc | bir_is_valid_pc (BirProgram p) pc} SUBSET (BIGUNION (IMAGE pcs_of_block (set p)))` by (
+   Q.UNABBREV_TAC `pcs_of_block` >>
+   SIMP_TAC std_ss [SUBSET_DEF, GSPECIFICATION, IN_BIGUNION, IN_IMAGE,
+     PULL_EXISTS, IN_COUNT, bir_is_valid_pc_def] >>
+   Cases >>
+   SIMP_TAC (std_ss++bir_TYPES_ss) [GSYM arithmeticTheory.LESS_EQ_IFF_LESS_SUC,
+      bir_programcounter_t_component_equality] >>
+   REPEAT STRIP_TAC >>
+   Q.EXISTS_TAC `bl` >>
+   rename1 `bir_get_program_block_info_by_label _ l = _` >>
+   FULL_SIMP_TAC std_ss [bir_get_program_block_info_by_label_def,
+     INDEX_FIND_EQ_SOME_0] >>
+   METIS_TAC [listTheory.MEM_EL]
+) >>
+
+`FINITE (BIGUNION (IMAGE pcs_of_block (set p)))` suffices_by
+  METIS_TAC [SUBSET_FINITE] >>
+
+Q.UNABBREV_TAC `pcs_of_block` >>
+REPEAT (POP_ASSUM (K ALL_TAC)) >>
+MATCH_MP_TAC FINITE_BIGUNION >>
+SIMP_TAC std_ss [IN_IMAGE, IMAGE_FINITE, FINITE_COUNT,
+  listTheory.FINITE_LIST_TO_SET, PULL_EXISTS]);
+
+
+
+(* If we loop a block that is entered infinitely often exists *)
+val bir_exec_infinite_steps_fun_LOOPING_BLOCK_EXISTS = store_thm (
+"bir_exec_infinite_steps_fun_LOOPING_BLOCK_EXISTS",
+``!p st.
+   (!n. ~(bir_state_is_terminated (bir_exec_infinite_steps_fun p st n))) ==>
+   ?l. MEM l (bir_labels_of_program p) /\
+       INFINITE {i | (bir_exec_infinite_steps_fun p st i).bst_pc = bir_block_pc l}``,
+
+REPEAT STRIP_TAC >>
+`!n. bir_is_valid_pc p (bir_exec_infinite_steps_fun p st n).bst_pc` by (
+   ASM_SIMP_TAC std_ss [bir_exec_infinite_steps_fun_valid_pc] >>
+   CCONTR_TAC >>
+   `~(bir_state_is_terminated st)` by METIS_TAC[bir_exec_infinite_steps_fun_REWRS] >>
+   `bir_state_is_terminated (bir_exec_infinite_steps_fun p st (SUC 0))` suffices_by METIS_TAC[] >>
+   SIMP_TAC std_ss [bir_exec_infinite_steps_fun_REWRS] >>
+   FULL_SIMP_TAC std_ss [
+     bir_exec_step_state_def, bir_exec_step_def, GSYM bir_get_current_statement_IS_SOME] >>
+   SIMP_TAC (std_ss++holBACore_ss) [bir_state_set_failed_def]
+) >>
+
+Q.ABBREV_TAC `index_set_of_pc = \pc. {i | (bir_exec_infinite_steps_fun p st i).bst_pc = pc}` >>
+
+`?pc. bir_is_valid_pc p pc /\ INFINITE (index_set_of_pc pc)` by (
+  CCONTR_TAC >>
+  `UNIV SUBSET (BIGUNION (IMAGE index_set_of_pc {pc | bir_is_valid_pc p pc}))` by (
+     Q.UNABBREV_TAC `index_set_of_pc` >>
+     ASM_SIMP_TAC std_ss [SUBSET_DEF, IN_UNIV, IN_BIGUNION, IN_IMAGE, PULL_EXISTS,
+       GSPECIFICATION]
+  ) >>
+  `FINITE (BIGUNION (IMAGE index_set_of_pc {pc | bir_is_valid_pc p pc}))` suffices_by
+     METIS_TAC [SUBSET_FINITE, INFINITE_NUM_UNIV] >>
+
+  MATCH_MP_TAC FINITE_BIGUNION >>
+  FULL_SIMP_TAC std_ss [IN_IMAGE, PULL_EXISTS, IMAGE_FINITE,
+    bir_is_valid_pc_FINITE, GSPECIFICATION] >>
+  METIS_TAC[]
+) >>
+
+
+Q.ABBREV_TAC `pc_set = index_set_of_pc pc DIFF (count pc.bpc_index)` >>
+`INFINITE pc_set` by METIS_TAC[FINITE_DIFF_down, FINITE_COUNT] >>
+
+Q.PAT_X_ASSUM `INFINITE (index_set_of_pc pc)` (K ALL_TAC) >>
+Q.UNABBREV_TAC `index_set_of_pc` >>
+
+`INFINITE (IMAGE (\i. i - pc.bpc_index) pc_set)` by (
+  `!x. FINITE {y | x = (\i. i - pc.bpc_index) y}` suffices_by
+     METIS_TAC[FINITELY_INJECTIVE_IMAGE_FINITE] >>
+
+  Tactical.REVERSE (Cases_on `x`) >- (
+     SIMP_TAC arith_ss [] >>
+     rename1 `SUC x' = _` >>
+     `{(y:num) | SUC x' = (y - pc.bpc_index)} = {SUC x' + pc.bpc_index}` suffices_by
+        SIMP_TAC std_ss [FINITE_SING] >>
+     SIMP_TAC arith_ss [EXTENSION, GSPECIFICATION, IN_SING]
+  ) >>
+  SIMP_TAC arith_ss [] >>
+  `{y | y <= pc.bpc_index} = count (SUC pc.bpc_index)` suffices_by SIMP_TAC std_ss [FINITE_COUNT] >>
+  SIMP_TAC arith_ss [EXTENSION, GSPECIFICATION, IN_COUNT]
+) >>
+
+Q.EXISTS_TAC `pc.bpc_label` >>
+ASM_SIMP_TAC std_ss [bir_is_valid_pc_label_OK] >>
+`IMAGE (\i. i - pc.bpc_index) pc_set SUBSET
+ {(i : num) | (bir_exec_infinite_steps_fun p st i).bst_pc = bir_block_pc pc.bpc_label}`
+  suffices_by METIS_TAC[SUBSET_FINITE] >>
+
+Q.UNABBREV_TAC `pc_set` >>
+REPEAT (Q.PAT_X_ASSUM `INFINITE _` (K ALL_TAC)) >>
+
+SIMP_TAC arith_ss [SUBSET_DEF, IN_DIFF, IN_COUNT, GSPECIFICATION, bir_block_pc_def,
+  IN_IMAGE, PULL_EXISTS] >>
+REPEAT STRIP_TAC >>
+MP_TAC (Q.SPECL [`p`, `st`, `i`] bir_exec_infinite_steps_fun_block_starts_at_front) >>
+ASM_SIMP_TAC arith_ss [] >>
+
+SIMP_TAC (std_ss++bir_TYPES_ss) [bir_programcounter_t_component_equality]);
+
+
+
+
+val bir_exec_infinite_steps_fun_PC_COND_SET_BLOCK_PC = store_thm (
+"bir_exec_infinite_steps_fun_PC_COND_SET_BLOCK_PC",
+``!p pc_cond st.
+   (!pc. (pc.bpc_index = 0) ==> pc_cond pc) ==>
+   (!n. ~(bir_state_is_terminated (bir_exec_infinite_steps_fun p st n))) ==>
+   INFINITE (bir_exec_infinite_steps_fun_PC_COND_SET pc_cond p st)``,
+
+REPEAT GEN_TAC >>
+STRIP_TAC >> STRIP_TAC >>
+MP_TAC (Q.SPECL [`p`, `st`] bir_exec_infinite_steps_fun_LOOPING_BLOCK_EXISTS) >>
+ASM_SIMP_TAC std_ss [] >>
+STRIP_TAC >>
+
+`({i | (bir_exec_infinite_steps_fun p st i).bst_pc = bir_block_pc l} DIFF {0})
+ SUBSET (bir_exec_infinite_steps_fun_PC_COND_SET pc_cond p st)`
+  suffices_by METIS_TAC[SUBSET_FINITE, FINITE_DIFF_down, FINITE_SING] >>
+
+FULL_SIMP_TAC (std_ss++bir_TYPES_ss) [SUBSET_DEF, IN_DIFF, IN_SING, GSPECIFICATION,
+  bir_block_pc_def, bir_exec_infinite_steps_fun_PC_COND_SET_def,
+  bir_state_COUNT_PC_def, bir_state_is_terminated_def]);
+
+
+
+
 (***************************************)
 (* bir_exec_infinite_steps_COUNT_STEPS *)
 (***************************************)
 
 val bir_exec_infinite_steps_COUNT_STEPS_UNFOLD = store_thm (
   "bir_exec_infinite_steps_COUNT_STEPS_UNFOLD",
-  ``!p st.
-    (bir_exec_infinite_steps_COUNT_STEPS p st =
-     if bir_state_is_terminated st then SOME 0 else
-     OPT_NUM_SUC (bir_exec_infinite_steps_COUNT_STEPS p (bir_exec_step_state p st)))``,
+  ``!pc_cond max_steps_opt p st.
+    (bir_exec_infinite_steps_COUNT_STEPS pc_cond max_steps_opt p st =
+     if (bir_state_is_terminated st \/ (max_steps_opt = SOME 0)) then SOME 0 else
+     (let st' = bir_exec_step_state p st in
+      let max_steps_opt' = if (bir_state_COUNT_PC pc_cond st') then OPT_NUM_PRE max_steps_opt else max_steps_opt in
+      OPT_NUM_SUC (bir_exec_infinite_steps_COUNT_STEPS pc_cond max_steps_opt' p st')))``,
 
 SIMP_TAC std_ss [bir_exec_infinite_steps_COUNT_STEPS_def,
   whileTheory.OLEAST_def] >>
 REPEAT GEN_TAC >>
-Q.ABBREV_TAC `P = \st i. bir_state_is_terminated (bir_exec_infinite_steps_fun p st i)` >>
-`(bir_state_is_terminated st = P st 0) /\ (!i. (P (bir_exec_step_state p st) i = P st (SUC i)))` by (
+Q.ABBREV_TAC `P = \max_steps_opt st i.
+   (bir_state_is_terminated (bir_exec_infinite_steps_fun p st i) \/
+   (max_steps_opt = SOME (bir_exec_infinite_steps_fun_COUNT_PCs pc_cond p st i)))` >>
+`(bir_state_is_terminated st \/  (max_steps_opt = SOME 0)) = P max_steps_opt st 0` by (
   Q.UNABBREV_TAC `P` >>
-  SIMP_TAC std_ss [bir_exec_infinite_steps_fun_REWRS]
+  SIMP_TAC std_ss [bir_exec_infinite_steps_fun_REWRS,
+    bir_exec_infinite_steps_fun_COUNT_PCs_def]
 ) >>
-ASM_SIMP_TAC std_ss [] >>
+
+`!i. ~(P max_steps_opt st 0) ==> (
+     (P (if bir_state_COUNT_PC pc_cond  (bir_exec_step_state p st) then OPT_NUM_PRE max_steps_opt
+        else max_steps_opt) (bir_exec_step_state p st) i) =
+      P max_steps_opt st (SUC i))` by (
+  Q.UNABBREV_TAC `P` >>
+  FULL_SIMP_TAC (std_ss++boolSimps.EQUIV_EXTRACT_ss) [bir_exec_infinite_steps_fun_REWRS,
+    bir_exec_infinite_steps_fun_COUNT_PCs_def, LET_DEF] >>
+  REPEAT STRIP_TAC >>
+  Cases_on `max_steps_opt` >> SIMP_TAC std_ss [OPT_NUM_PRE_def] >>
+  rename1 `SOME max_steps <> SOME 0`  >>
+  FULL_SIMP_TAC std_ss [] >>
+  Cases_on `max_steps` >- FULL_SIMP_TAC std_ss [] >>
+  rename1 `SUC max_steps' <> 0` >>
+  Cases_on `bir_state_COUNT_PC pc_cond (bir_exec_step_state p st)` >> (
+    ASM_SIMP_TAC std_ss []
+  )
+) >>
+ASM_SIMP_TAC std_ss [LET_DEF] >>
 REPEAT (POP_ASSUM (K ALL_TAC)) >>
 Tactical.REVERSE COND_CASES_TAC >- (
   FULL_SIMP_TAC std_ss [OPT_NUM_SUC_def]
 ) >>
 FULL_SIMP_TAC std_ss [] >>
-Cases_on `P st 0` >- (
+Cases_on `P max_steps_opt st 0` >- (
   ASM_SIMP_TAC std_ss [] >>
   MATCH_MP_TAC bitTheory.LEAST_THM >>
   ASM_SIMP_TAC std_ss []
@@ -118,39 +612,78 @@ MATCH_MP_TAC LEAST_SUC >>
 METIS_TAC[]);
 
 
-val bir_exec_infinite_steps_COUNT_STEPS_TERMINATED_REWRS = store_thm (
-  "bir_exec_infinite_steps_COUNT_STEPS_TERMINATED_REWRS",
-  ``(!p st.
+val bir_exec_infinite_steps_COUNT_STEPS_TERMINATED_REWR = store_thm (
+  "bir_exec_infinite_steps_COUNT_STEPS_TERMINATED_REWR",
+  ``!pc_cond max_steps p st.
     bir_state_is_terminated st ==>
-    (bir_exec_infinite_steps_COUNT_STEPS p st = SOME 0)) /\
+    (bir_exec_infinite_steps_COUNT_STEPS pc_cond max_steps p st = SOME 0)``,
 
-   (!p st.
-    ~(bir_state_is_terminated st) ==>
-    (bir_exec_infinite_steps_COUNT_STEPS p st =
-    (OPT_NUM_SUC (bir_exec_infinite_steps_COUNT_STEPS p (bir_exec_step_state p st)))))``,
-
-CONJ_TAC >> SIMP_TAC std_ss [Once bir_exec_infinite_steps_COUNT_STEPS_UNFOLD]);
+SIMP_TAC std_ss [Once bir_exec_infinite_steps_COUNT_STEPS_UNFOLD]);
 
 
-val bir_exec_infinite_steps_COUNT_STEPS_EQ_NONE = store_thm ("bir_exec_infinite_steps_COUNT_STEPS_EQ_NONE",
-  ``(bir_exec_infinite_steps_COUNT_STEPS p state = NONE) <=>
-    (!n. ~(bir_state_is_terminated (bir_exec_infinite_steps_fun p state n)))``,
+val bir_exec_infinite_steps_COUNT_STEPS_NO_STEPS_REWR = store_thm (
+  "bir_exec_infinite_steps_COUNT_STEPS_NO_STEPS_REWR",
+  ``!pc_cond p st.
+    (bir_exec_infinite_steps_COUNT_STEPS pc_cond (SOME 0) p st = SOME 0)``,
 
-SIMP_TAC std_ss [bir_exec_infinite_steps_COUNT_STEPS_def, whileTheory.OLEAST_def]);
+SIMP_TAC std_ss [Once bir_exec_infinite_steps_COUNT_STEPS_UNFOLD]);
+
+
+val bir_exec_infinite_steps_COUNT_STEPS_STEP_REWR = store_thm (
+ "bir_exec_infinite_steps_COUNT_STEPS_STEP_REWR",
+``!pc_cond p st max_steps.
+    ~(bir_state_is_terminated st) /\ ~(max_steps = SOME 0) ==>
+
+    (bir_exec_infinite_steps_COUNT_STEPS pc_cond max_steps p st =
+    (let st' = bir_exec_step_state p st in
+    let max_steps_opt' =
+          if bir_state_COUNT_PC pc_cond st' then OPT_NUM_PRE max_steps
+          else max_steps
+    in
+      OPT_NUM_SUC
+        (bir_exec_infinite_steps_COUNT_STEPS pc_cond max_steps_opt' p
+           st')))``,
+
+SIMP_TAC std_ss [Once bir_exec_infinite_steps_COUNT_STEPS_UNFOLD]);
 
 
 val bir_exec_infinite_steps_COUNT_STEPS_EQ_SOME = store_thm ("bir_exec_infinite_steps_COUNT_STEPS_EQ_SOME",
-  ``(bir_exec_infinite_steps_COUNT_STEPS p state = SOME i) <=>
-    ((bir_state_is_terminated (bir_exec_infinite_steps_fun p state i)) /\
-     (!n. n < i ==> ~(bir_state_is_terminated (bir_exec_infinite_steps_fun p state n))))``,
+  ``(bir_exec_infinite_steps_COUNT_STEPS pc_cond max_steps_opt p state = SOME i) <=>
+    ((!n. n < i ==> ~(bir_state_is_terminated (bir_exec_infinite_steps_fun p state n)) /\
+                    (max_steps_opt <> SOME
+           (bir_exec_infinite_steps_fun_COUNT_PCs pc_cond p state n))) /\
+    ((bir_state_is_terminated (bir_exec_infinite_steps_fun p state i)) \/
+    (max_steps_opt = SOME (bir_exec_infinite_steps_fun_COUNT_PCs pc_cond p state i))))``,
 
 SIMP_TAC std_ss [bir_exec_infinite_steps_COUNT_STEPS_def, whileTheory.OLEAST_def] >>
-Q.ABBREV_TAC `P = (\state i. bir_state_is_terminated ((bir_exec_infinite_steps_fun p state i)))` >>
+Q.ABBREV_TAC `P = (\max_steps_opt state i.
+   (bir_state_is_terminated ((bir_exec_infinite_steps_fun p state i))) \/
+   (max_steps_opt =
+      SOME (bir_exec_infinite_steps_fun_COUNT_PCs pc_cond p state i)))` >>
+`!n. (~bir_state_is_terminated (bir_exec_infinite_steps_fun p state n) /\
+     (max_steps_opt <> SOME (bir_exec_infinite_steps_fun_COUNT_PCs pc_cond p state n))) =
+     ~(P max_steps_opt state n)` by (
+  Q.UNABBREV_TAC `P` >> SIMP_TAC std_ss []) >>
 ASM_SIMP_TAC std_ss [] >> POP_ASSUM (K ALL_TAC) >>
 EQ_TAC >> STRIP_TAC >| [
   METIS_TAC[whileTheory.LEAST_EXISTS_IMP],
   METIS_TAC[bitTheory.LEAST_THM]
 ]);
+
+
+val bir_exec_infinite_steps_COUNT_STEPS_EQ_NONE = store_thm (
+ "bir_exec_infinite_steps_COUNT_STEPS_EQ_NONE",
+  ``(bir_exec_infinite_steps_COUNT_STEPS pc_cond max_steps_opt p state = NONE) <=>
+    (!n. ~(bir_state_is_terminated (bir_exec_infinite_steps_fun p state n))) /\
+    (case max_steps_opt of NONE => T | SOME max_steps =>
+       (!i. bir_exec_infinite_steps_fun_COUNT_PCs pc_cond p state i < max_steps))``,
+
+SIMP_TAC std_ss [bir_exec_infinite_steps_COUNT_STEPS_def, whileTheory.OLEAST_def] >>
+SIMP_TAC (std_ss++boolSimps.EQUIV_EXTRACT_ss) [FORALL_AND_THM] >>
+STRIP_TAC >>
+Cases_on `max_steps_opt` >> SIMP_TAC std_ss [] >>
+METIS_TAC[bir_exec_infinite_steps_fun_COUNT_PCs_COMPLETE_FORALL_NEQ]);
+
 
 
 (***************************************)
@@ -167,7 +700,7 @@ SIMP_TAC arith_ss [bir_exec_steps_observe_llist_NEQ_SOME0, OPT_NUM_PRE_def]);
 
 
 val bir_exec_steps_observe_llist_NONE = store_thm ("bir_exec_steps_observe_llist_NONE",
- ``!p st n. bir_exec_steps_observe_llist p st NONE =
+ ``!p st. bir_exec_steps_observe_llist p st NONE =
             (let (fe, st') = bir_exec_step p st in
              let ll' = bir_exec_steps_observe_llist p st' NONE in
              (OPT_LCONS fe ll'))``,
@@ -375,143 +908,365 @@ ASM_SIMP_TAC std_ss [bir_exec_steps_observe_list_to_llist_THE,
 
 
 (***************************************************************)
-(* bir_exec_steps_opt                                          *)
+(* bir_exec_steps_GEN                                          *)
 (***************************************************************)
 
-val bir_exec_steps_opt_REWR_TERMINATED = store_thm ("bir_exec_steps_opt_REWR_TERMINATED",
-  ``!p st max_steps.
+val bir_exec_steps_GEN_REWR_TERMINATED = store_thm ("bir_exec_steps_GEN_REWR_TERMINATED",
+  ``!p st pc_cond max_steps.
     bir_state_is_terminated st ==>
-    (bir_exec_steps_opt p st max_steps = ([||], SOME (0, st)))``,
+    (bir_exec_steps_GEN pc_cond p st max_steps = BER_Ended [] 0 0 st)``,
 
-SIMP_TAC std_ss [bir_exec_steps_opt_def, bir_exec_infinite_steps_COUNT_STEPS_TERMINATED_REWRS,
-  OPT_NUM_MIN_SOME0, bir_exec_steps_observe_llist_0, LET_DEF,
-  bir_exec_infinite_steps_fun_REWRS]);
-
-
-val bir_exec_steps_opt_no_steps = store_thm ("bir_exec_steps_opt_no_steps",
-  ``!p st.
-    (bir_exec_steps_opt p st (SOME 0) = ([||], SOME (0, st)))``,
-
-SIMP_TAC std_ss [bir_exec_steps_opt_def,
-  OPT_NUM_MIN_SOME0, LET_THM, bir_exec_steps_observe_llist_0,
-  bir_exec_infinite_steps_fun_REWRS]);
+SIMP_TAC std_ss [bir_exec_steps_GEN_def,
+ bir_exec_infinite_steps_COUNT_STEPS_TERMINATED_REWR,
+  bir_exec_steps_observe_llist_0, LET_DEF,
+  bir_exec_infinite_steps_fun_REWRS, toList_THM,
+  bir_exec_infinite_steps_fun_COUNT_PCs_def]);
 
 
-val bir_exec_steps_opt_REWR_NOT_TERMINATED = store_thm ("bir_exec_steps_opt_REWR_NOT_TERMINATED",
-  ``!p st max_steps.
+val bir_exec_steps_GEN_REWR_no_steps = store_thm ("bir_exec_steps_GEN_REWR_no_steps",
+  ``!pc_cond p st.
+    (bir_exec_steps_GEN pc_cond p st (SOME 0) = BER_Ended [] 0 0 st)``,
+
+SIMP_TAC std_ss [bir_exec_steps_GEN_def,
+  bir_exec_infinite_steps_COUNT_STEPS_NO_STEPS_REWR,
+  bir_exec_steps_observe_llist_0, LET_DEF,
+  bir_exec_infinite_steps_fun_REWRS, toList_THM,
+  bir_exec_infinite_steps_fun_COUNT_PCs_def]);
+
+
+val bir_exec_steps_GEN_REWR_STEP = store_thm ("bir_exec_steps_GEN_REWR_STEP",
+  ``!pc_cond p st max_steps.
     ~(bir_state_is_terminated st) ==>
-    (bir_exec_steps_opt p st max_steps =
-      (if (max_steps = SOME 0) then ([||], SOME (0, st)) else (
+    (bir_exec_steps_GEN pc_cond p st max_steps =
+      (if (max_steps = SOME 0) then BER_Ended [] 0 0 st else (
       (let (fe, st') = bir_exec_step p st in
-       let (ll, fst_opt) = (bir_exec_steps_opt p st' (OPT_NUM_PRE max_steps)) in
-       ((OPT_LCONS fe ll),
-          OPTION_MAP (\ (i, st). (SUC i, st)) fst_opt)))))``,
+       let max_steps' = if (bir_state_COUNT_PC pc_cond st') then (OPT_NUM_PRE max_steps) else max_steps in
+       (case (bir_exec_steps_GEN pc_cond p st' max_steps') of
+             BER_Ended ol step_count pc_count st_final =>
+             BER_Ended (OPT_CONS fe ol) (SUC step_count)
+                       (if (bir_state_COUNT_PC pc_cond st') then SUC pc_count else pc_count) st_final
+           | BER_Looping oll => BER_Looping (OPT_LCONS fe oll))))))``,
 
 REPEAT GEN_TAC >>
-Cases_on `max_steps = SOME 0` >- ASM_SIMP_TAC std_ss [bir_exec_steps_opt_no_steps] >>
+Cases_on `max_steps = SOME 0` >- ASM_SIMP_TAC std_ss [bir_exec_steps_GEN_REWR_no_steps] >>
 `?fe st'. bir_exec_step p st = (fe, st')` by METIS_TAC[pairTheory.PAIR] >>
-ASM_SIMP_TAC std_ss [bir_exec_steps_opt_def, bir_exec_infinite_steps_COUNT_STEPS_TERMINATED_REWRS] >>
+ASM_SIMP_TAC std_ss [bir_exec_steps_GEN_def, bir_exec_infinite_steps_COUNT_STEPS_STEP_REWR] >>
 
-ASM_SIMP_TAC std_ss [bir_exec_step_state_def, OPT_NUM_MIN_OPT_NUM_SUC, LET_THM,
+ASM_SIMP_TAC std_ss [bir_exec_step_state_def, LET_THM,
   bir_exec_steps_observe_llist_OPT_NUM_SUC] >>
-Q.ABBREV_TAC `no = OPT_NUM_MIN (OPT_NUM_PRE max_steps)
-        (bir_exec_infinite_steps_COUNT_STEPS p st')` >>
+Q.ABBREV_TAC `no = (bir_exec_infinite_steps_COUNT_STEPS pc_cond
+         (if bir_state_COUNT_PC pc_cond st' then OPT_NUM_PRE max_steps
+          else max_steps) p st')` >>
 Cases_on `no` >> (
-  ASM_SIMP_TAC std_ss [OPT_NUM_SUC_def, bir_exec_infinite_steps_fun_REWRS,
+  ASM_SIMP_TAC (std_ss++bir_TYPES_ss) [OPT_NUM_SUC_def, bir_exec_infinite_steps_fun_REWRS,
     bir_exec_step_state_def]
+) >>
+
+ASM_SIMP_TAC std_ss [bir_exec_infinite_steps_fun_COUNT_PCs_def, LET_THM, bir_exec_step_state_def] >>
+Cases_on `fe` >> (
+  SIMP_TAC std_ss [bir_exec_steps_observe_llist_toList_SOME, OPT_LCONS_def,
+    OPT_CONS_def, toList_THM]
 ));
 
 
-val bir_exec_steps_opt_EQ_NONE = store_thm ("bir_exec_steps_opt_EQ_NONE",
-  ``((bir_exec_steps_opt p state mo) = (ll, NONE)) <=>
+val bir_exec_steps_GEN_EQ_Looping = store_thm ("bir_exec_steps_GEN_EQ_Looping",
+  ``((bir_exec_steps_GEN pc_cond p state mo) = BER_Looping ll) <=>
     ((ll = bir_exec_steps_observe_llist p state NONE) /\
-     (mo = NONE) /\ (bir_exec_infinite_steps_COUNT_STEPS p state = NONE))``,
+     (bir_exec_infinite_steps_COUNT_STEPS pc_cond mo p state = NONE))``,
 
-Cases_on `mo` >> Cases_on `bir_exec_infinite_steps_COUNT_STEPS p state` >> (
-  ASM_SIMP_TAC (std_ss++boolSimps.EQUIV_EXTRACT_ss) [bir_exec_steps_opt_def, LET_DEF, OPT_NUM_MIN_REWRS]
+Cases_on `bir_exec_infinite_steps_COUNT_STEPS pc_cond mo p state` >> (
+  ASM_SIMP_TAC (std_ss++bir_TYPES_ss++boolSimps.EQUIV_EXTRACT_ss) [bir_exec_steps_GEN_def, LET_DEF]
 ));
 
 
-val bir_exec_steps_opt_EQ_NONE_SND = store_thm ("bir_exec_steps_opt_EQ_NONE_SND",
-  ``(SND (bir_exec_steps_opt p state mo) = NONE) <=>
-    (
-     (mo = NONE) /\ (bir_exec_infinite_steps_COUNT_STEPS p state = NONE))``,
+(* Together with the theorems about the infinity of
+   bir_exec_infinite_steps_fun_PC_COND_SET, we can derive easily, that we
+   do terminate, if a step number was given and we count at least when entering a new block. *)
 
-Cases_on `mo` >> Cases_on `bir_exec_infinite_steps_COUNT_STEPS p state` >> (
-  ASM_SIMP_TAC (std_ss++boolSimps.EQUIV_EXTRACT_ss) [bir_exec_steps_opt_def, LET_DEF, OPT_NUM_MIN_REWRS]
-));
+val bir_exec_steps_GEN_NOT_Looping_max_steps_blocks = store_thm (
+ "bir_exec_steps_GEN_NOT_Looping_max_steps_blocks",
+``!pc_cond p state m.
+  (!pc. (pc.bpc_index = 0) ==> pc_cond pc) ==>
+  IS_BER_Ended (bir_exec_steps_GEN pc_cond p state (SOME m))``,
+
+REPEAT STRIP_TAC >>
+Cases_on `bir_exec_steps_GEN pc_cond p state (SOME m)` >> (
+  SIMP_TAC std_ss [IS_BER_Ended_def]
+) >>
+FULL_SIMP_TAC std_ss [bir_exec_steps_GEN_EQ_Looping,
+  bir_exec_infinite_steps_COUNT_STEPS_EQ_NONE,
+  GSYM FINITE_bir_exec_infinite_steps_fun_PC_COND_SET] >>
+METIS_TAC[bir_exec_infinite_steps_fun_PC_COND_SET_BLOCK_PC]);
 
 
-val bir_exec_steps_opt_EQ_SOME = store_thm ("bir_exec_steps_opt_EQ_SOME",
-  ``!p state mo ll c state'.
-    (bir_exec_steps_opt p state mo = (ll, SOME (c, state'))) <=>
-    ((ll = bir_exec_steps_observe_llist p state (SOME c)) /\
+
+val bir_exec_steps_GEN_EQ_Ended = store_thm ("bir_exec_steps_GEN_EQ_Ended",
+  ``!p state mo ol step_c pc_c state' pc_cond.
+    (bir_exec_steps_GEN pc_cond p state mo = BER_Ended ol step_c pc_c state') <=>
+    ((ol = bir_exec_steps_observe_list p state step_c) /\
+     (pc_c = bir_exec_infinite_steps_fun_COUNT_PCs pc_cond p state step_c) /\
      (case mo of NONE => (bir_state_is_terminated state')
-               | SOME m => ((c <= m) /\ ((c < m) ==> (bir_state_is_terminated state')))) /\
-     (state' = bir_exec_infinite_steps_fun p state c) /\
-     (!n. n < c ==> ~(bir_state_is_terminated (bir_exec_infinite_steps_fun p state n))))``,
+               | SOME m => ((pc_c <= m) /\ ((pc_c < m) ==> (bir_state_is_terminated state')) /\
+                            (((pc_c = m) /\ (0 < m)) ==> (
+                               bir_state_COUNT_PC pc_cond state')))) /\
+     (state' = bir_exec_infinite_steps_fun p state step_c) /\
+     (!n. n < step_c ==> (~(bir_state_is_terminated (bir_exec_infinite_steps_fun p state n)) /\
+                          mo <> SOME (bir_exec_infinite_steps_fun_COUNT_PCs pc_cond p state n))))``,
 
 REPEAT GEN_TAC >>
 EQ_TAC >- (
-  SIMP_TAC std_ss [bir_exec_steps_opt_def, LET_DEF] >>
-  Cases_on ` OPT_NUM_MIN mo (bir_exec_infinite_steps_COUNT_STEPS p state)` >> (
-    ASM_SIMP_TAC std_ss []
+  SIMP_TAC std_ss [bir_exec_steps_GEN_def, LET_DEF] >>
+  Cases_on `bir_exec_infinite_steps_COUNT_STEPS pc_cond mo p state` >> (
+    ASM_SIMP_TAC (std_ss++bir_TYPES_ss) []
   ) >>
   STRIP_TAC >> REPEAT (BasicProvers.VAR_EQ_TAC) >>
-  ASM_REWRITE_TAC[] >>
-  Cases_on `(bir_exec_infinite_steps_COUNT_STEPS p state)` >- (
-    FULL_SIMP_TAC std_ss [bir_exec_infinite_steps_COUNT_STEPS_EQ_NONE, OPT_NUM_MIN_REWRS]
-  ) >>
-  rename1 `bir_exec_infinite_steps_COUNT_STEPS _ _ = SOME cc2` >>
-  `(c <= cc2) /\ (c <> cc2 ==> (mo = SOME c)) /\ (!c'. (mo = SOME c') ==> c <= c')` by (
-     Cases_on `mo` >>
-     FULL_SIMP_TAC arith_ss [OPT_NUM_MIN_REWRS] >>
-     BasicProvers.VAR_EQ_TAC >>
-     SIMP_TAC arith_ss [arithmeticTheory.MIN_DEF]
-  ) >>
-  FULL_SIMP_TAC arith_ss [bir_exec_infinite_steps_COUNT_STEPS_EQ_SOME] >>
-  Cases_on `mo` >> (
-    FULL_SIMP_TAC arith_ss []
-  ) >>
-  STRIP_TAC >>
-  rename1 `c < cc1` >>
-  `cc1 <> c` by DECIDE_TAC >>
-  FULL_SIMP_TAC std_ss []
-) >- (
-  SIMP_TAC std_ss [bir_exec_steps_opt_def, LET_DEF] >>
-  STRIP_TAC >> REPEAT (BasicProvers.VAR_EQ_TAC) >>
+  ASM_SIMP_TAC std_ss [bir_exec_steps_observe_llist_toList_SOME] >>
+  Q.PAT_X_ASSUM `_ = SOME step_c` MP_TAC >>
+  SIMP_TAC std_ss [bir_exec_infinite_steps_COUNT_STEPS_EQ_SOME] >>
+  Q.HO_MATCH_ABBREV_TAC `(_ /\ P step_c mo) ==> _` >>
+  REPEAT STRIP_TAC >>
   Cases_on `mo` >- (
-    FULL_SIMP_TAC arith_ss [OPT_NUM_MIN_REWRS] >>
-    `bir_exec_infinite_steps_COUNT_STEPS p state = SOME c` by
-      METIS_TAC[bir_exec_infinite_steps_COUNT_STEPS_EQ_SOME] >>
-    ASM_SIMP_TAC std_ss []
+    Q.UNABBREV_TAC `P` >>
+    FULL_SIMP_TAC std_ss []
   ) >>
-  rename1 `OPT_NUM_MIN (SOME cc1) _` >>
-  FULL_SIMP_TAC std_ss [] >>
-  Cases_on `bir_exec_infinite_steps_COUNT_STEPS p state` >- (
-    ASM_SIMP_TAC std_ss [OPT_NUM_MIN_REWRS] >>
+  FULL_SIMP_TAC std_ss [FORALL_AND_THM, IMP_CONJ_THM] >>
+  Cases_on `step_c` >- (
+    Q.UNABBREV_TAC `P` >>
+    FULL_SIMP_TAC (std_ss++boolSimps.CONJ_ss) [bir_exec_infinite_steps_fun_COUNT_PCs_def]
+  ) >>
+  rename1 `P (SUC step_c') (SOME m)` >>
+  `bir_exec_infinite_steps_fun_COUNT_PCs pc_cond p state step_c' < m` by (
+     CCONTR_TAC >>
+     FULL_SIMP_TAC std_ss [arithmeticTheory.NOT_LESS, GSYM arithmeticTheory.LESS_EQ_IFF_LESS_SUC] >>
+     METIS_TAC[bir_exec_infinite_steps_fun_COUNT_PCs_COMPLETE_LESS_EQ]
+  ) >>
+  ASM_SIMP_TAC (arith_ss++boolSimps.LIFT_COND_ss) [bir_exec_infinite_steps_fun_COUNT_PCs_END_DEF, LET_DEF] >>
+  Q.UNABBREV_TAC `P` >> (
+    FULL_SIMP_TAC std_ss []
+  ) >>
+  FULL_SIMP_TAC std_ss [bir_exec_infinite_steps_fun_COUNT_PCs_END_DEF, LET_DEF] >>
+  Cases_on `bir_state_COUNT_PC pc_cond
+          (bir_exec_infinite_steps_fun p state (SUC step_c'))` >> (
+    FULL_SIMP_TAC arith_ss []
+  )
+) >- (
+  SIMP_TAC std_ss [bir_exec_steps_GEN_def, LET_DEF] >>
+  REPEAT STRIP_TAC >>
+  REPEAT BasicProvers.VAR_EQ_TAC >>
+  Cases_on ` bir_exec_infinite_steps_COUNT_STEPS pc_cond mo p state` >- (
+    SIMP_TAC (std_ss++bir_TYPES_ss) [] >>
     FULL_SIMP_TAC std_ss [bir_exec_infinite_steps_COUNT_STEPS_EQ_NONE] >>
-    `cc1 = c` by DECIDE_TAC >>
-    ASM_REWRITE_TAC[]
+    Cases_on `mo` >> FULL_SIMP_TAC std_ss [] >>
+    rename1 `_ <= (m:num)` >>
+    `m = bir_exec_infinite_steps_fun_COUNT_PCs pc_cond p state step_c` by DECIDE_TAC >>
+    METIS_TAC[FINITE_bir_exec_infinite_steps_fun_PC_COND_SET]
   ) >>
-  rename1 `OPT_NUM_MIN (SOME cc1) (SOME cc2)` >>
-  ASM_SIMP_TAC std_ss [OPT_NUM_MIN_REWRS] >>
-  `MIN cc1 cc2 = c` suffices_by SIMP_TAC std_ss [] >>
-  FULL_SIMP_TAC arith_ss [bir_exec_infinite_steps_COUNT_STEPS_EQ_SOME] >>
-  `~(cc2 < c)` by METIS_TAC[] >>
-  Cases_on `c < cc1` >| [
-    `~(c < cc2)` by METIS_TAC[] >>
-    `c = cc2` by DECIDE_TAC >>
-    FULL_SIMP_TAC arith_ss [arithmeticTheory.MIN_DEF],
-
-    FULL_SIMP_TAC arith_ss [arithmeticTheory.MIN_DEF]
-  ]
+  rename1 `_ = SOME (step_c':num)` >>
+  FULL_SIMP_TAC (std_ss++bir_TYPES_ss) [bir_exec_steps_observe_llist_toList_SOME] >>
+  `step_c' = step_c` suffices_by METIS_TAC[] >>
+  Q.PAT_X_ASSUM `_ = SOME step_c'` MP_TAC >>
+  FULL_SIMP_TAC std_ss [bir_exec_infinite_steps_COUNT_STEPS_EQ_SOME] >>
+  Q.HO_MATCH_ABBREV_TAC `(_ /\ P step_c' mo) ==> _` >>
+  REPEAT STRIP_TAC >>
+  Cases_on `mo` >- (
+    Q.UNABBREV_TAC `P` >>
+    FULL_SIMP_TAC std_ss [] >>
+    `~(step_c < step_c')` by METIS_TAC[] >>
+    `~(step_c' < step_c)` by METIS_TAC[] >>
+    DECIDE_TAC
+  ) >>
+  rename1 `P _ (SOME m)` >>
+  FULL_SIMP_TAC std_ss [] >>
+  `~(step_c < step_c')` by (
+     CCONTR_TAC >>
+     Q.PAT_X_ASSUM `!n. n < step_c' ==> _` (MP_TAC o Q.SPEC `step_c`) >>
+     FULL_SIMP_TAC std_ss [] >>
+     METIS_TAC [arithmeticTheory.LESS_OR_EQ]
+  ) >>
+  `~(step_c' < step_c)` by (
+     CCONTR_TAC >>
+     Q.PAT_X_ASSUM `!n. n < step_c ==> _` (MP_TAC o Q.SPEC `step_c'`) >>
+     Q.UNABBREV_TAC `P` >>
+     FULL_SIMP_TAC std_ss []
+  ) >>
+  DECIDE_TAC
 ));
 
 
+
+val bir_exec_steps_GEN_EQ_Ended_0 = store_thm ("bir_exec_steps_GEN_EQ_Ended_0",
+  ``(!pc_cond p st max_steps ol c_pc st'.
+    (bir_exec_steps_GEN pc_cond p st max_steps = BER_Ended ol 0 c_pc st') <=> (
+       (ol = []) /\ (c_pc = 0) /\ (st' = st) /\
+       (bir_state_is_terminated st \/ (max_steps = SOME 0))))``,
+
+SIMP_TAC (std_ss++boolSimps.EQUIV_EXTRACT_ss) [bir_exec_steps_GEN_EQ_Ended,
+  bir_exec_infinite_steps_fun_COUNT_PCs_def, bir_exec_steps_observe_list_REWRS,
+  bir_exec_infinite_steps_fun_REWRS] >>
+Cases_on `max_steps` >> (
+  SIMP_TAC std_ss []
+) >>
+rename1 `0 < m` >>
+Cases_on `m` >> SIMP_TAC arith_ss []);
+
+
+
+val bir_exec_steps_GEN_EQ_Ended_SUC = store_thm ("bir_exec_steps_GEN_EQ_Ended_SUC",
+  ``(!pc_cond p st max_steps c_st ol c_pc st'.
+    (bir_exec_steps_GEN pc_cond p st max_steps = BER_Ended ol (SUC c_st) c_pc st') <=> (
+       ~(bir_state_is_terminated st) /\ (max_steps <> SOME 0) /\
+
+       let (fe, st1) = bir_exec_step p st in
+       let max_steps' = if bir_state_COUNT_PC pc_cond st1 then OPT_NUM_PRE max_steps else max_steps in
+       ?ol' c_pc'. (bir_exec_steps_GEN pc_cond p st1 max_steps' = BER_Ended ol' c_st c_pc' st') /\
+                   (ol = OPT_CONS fe ol') /\
+                   (c_pc = if (bir_state_COUNT_PC pc_cond st1) then SUC c_pc' else c_pc')))``,
+
+
+REPEAT STRIP_TAC >>
+Cases_on `bir_state_is_terminated st` >- (
+  ASM_SIMP_TAC (arith_ss++bir_TYPES_ss) [bir_exec_steps_GEN_REWR_TERMINATED]
+) >>
+Cases_on `max_steps = SOME 0` >- (
+  ASM_SIMP_TAC (arith_ss++bir_TYPES_ss) [bir_exec_steps_GEN_REWR_no_steps]
+) >>
+`?fe st1. bir_exec_step p st = (fe, st1)` by METIS_TAC[pairTheory.PAIR] >>
+ASM_SIMP_TAC std_ss [bir_exec_steps_GEN_REWR_STEP, LET_DEF] >>
+Q.ABBREV_TAC `max_steps' = if bir_state_COUNT_PC pc_cond st1 then OPT_NUM_PRE max_steps else max_steps` >>
+
+Tactical.REVERSE (Cases_on `bir_exec_steps_GEN pc_cond p st1 max_steps'`) >- (
+  SIMP_TAC (std_ss++bir_TYPES_ss) []
+) >>
+SIMP_TAC (std_ss++bir_TYPES_ss++boolSimps.EQUIV_EXTRACT_ss) []);
+
+
+
+
 (***************************************************************)
-(* bir_exec_steps_n                                            *)
+(* combine multiple runs                                       *)
 (***************************************************************)
+
+
+
+val bir_exec_steps_GEN_SOME_ADD_Ended = store_thm ("bir_exec_steps_GEN_SOME_ADD_Ended",
+  ``!n1 mo pc_count p state0 state1 state2 l1 l2 c_st1 c_st2 c_pc1 c_pc2.
+    (bir_exec_steps_GEN pc_count p state0 (SOME n1) = BER_Ended l1 c_pc1 c_st1 state1) ==>
+    (bir_exec_steps_GEN pc_count p state1 mo = BER_Ended l2 c_pc2 c_st2 state2) ==>
+    (bir_exec_steps_GEN pc_count p state0 (OPTION_MAP (\n2. n1+n2) mo) = BER_Ended (l1++l2)
+         (c_pc1+c_pc2) (c_st1 + c_st2) state2)``,
+
+SIMP_TAC arith_ss [bir_exec_steps_GEN_EQ_Ended,
+  GSYM bir_exec_steps_observe_list_ADD,
+  GSYM bir_exec_infinite_steps_fun_ADD,
+  bir_exec_infinite_steps_fun_COUNT_PCs_ADD] >>
+REPEAT GEN_TAC >> REPEAT DISCH_TAC >>
+FULL_SIMP_TAC std_ss [] >>
+Q.ABBREV_TAC `st1 = (bir_exec_infinite_steps_fun p state0 c_pc1)` >>
+Cases_on ` bir_exec_infinite_steps_fun_COUNT_PCs pc_count p state0 c_pc1 < n1` >- (
+  FULL_SIMP_TAC std_ss [] >>
+  Q.PAT_X_ASSUM `bir_state_is_terminated _` ASSUME_TAC >>
+  FULL_SIMP_TAC arith_ss [bir_exec_infinite_steps_fun_TERMINATED_0,
+    arithmeticTheory.NOT_LESS] >>
+  Tactical.REVERSE (Cases_on `c_pc2`) >- METIS_TAC[arithmeticTheory.NOT_SUC_LESS_EQ_0] >>
+  FULL_SIMP_TAC (std_ss++boolSimps.CONJ_ss) [bir_exec_infinite_steps_fun_COUNT_PCs_def] >>
+  Tactical.REVERSE CONJ_TAC >- (
+    REPEAT STRIP_TAC >>
+    DISJ2_TAC >>
+    `n1 <= n1 + n2` by DECIDE_TAC >>
+    METIS_TAC[bir_exec_infinite_steps_fun_COUNT_PCs_COMPLETE_LESS_EQ,
+      arithmeticTheory.LESS_EQ_LESS_TRANS]
+  ) >>
+  Cases_on `mo` >> FULL_SIMP_TAC arith_ss []
+) >>
+`bir_exec_infinite_steps_fun_COUNT_PCs pc_count p state0 c_pc1 = n1` by DECIDE_TAC >>
+FULL_SIMP_TAC arith_ss [GSYM bir_exec_infinite_steps_fun_ADD] >>
+Tactical.REVERSE CONJ_TAC >- (
+  GEN_TAC >> STRIP_TAC >>
+  rename1 `(n:num) < c_pc1 + _` >>
+  Cases_on `n < c_pc1` >- (
+    ASM_SIMP_TAC std_ss [] >>
+    GEN_TAC >> DISJ2_TAC >>
+    rename1 `_ <> (n1:num) + n2` >>
+    `n1 <= n1 + n2` by DECIDE_TAC >>
+    METIS_TAC[bir_exec_infinite_steps_fun_COUNT_PCs_COMPLETE_LESS_EQ,
+      arithmeticTheory.LESS_EQ_LESS_TRANS]
+  ) >>
+  `?n'. n = c_pc1 + n'` by METIS_TAC[arithmeticTheory.LESS_EQ_EXISTS, arithmeticTheory.NOT_LESS] >>
+  FULL_SIMP_TAC arith_ss [GSYM bir_exec_infinite_steps_fun_ADD,
+    bir_exec_infinite_steps_fun_COUNT_PCs_ADD]
+) >>
+Cases_on `mo` >> (
+  FULL_SIMP_TAC std_ss []
+) >>
+rename1 `0 < n1 + n2` >>
+Cases_on `n2 = 0` >- (
+  `c_pc2 = 0` by (
+     Q.PAT_X_ASSUM `!n. n < c_pc2 ==> _` (MP_TAC o Q.SPEC `0`) >>
+     ASM_SIMP_TAC arith_ss [bir_exec_infinite_steps_fun_COUNT_PCs_def]
+  ) >>
+  FULL_SIMP_TAC std_ss [bir_exec_infinite_steps_fun_REWRS]
+) >>
+FULL_SIMP_TAC arith_ss []);
+
+
+val bir_exec_steps_GEN_SOME_ADD_Looping = store_thm ("bir_exec_steps_GEN_SOME_ADD_Looping",
+  ``!n1 mo pc_count p state0 state1 l1 ll2 c_st1 c_pc1.
+    (bir_exec_steps_GEN pc_count p state0 (SOME n1) = BER_Ended l1 c_pc1 c_st1 state1) ==>
+    (bir_exec_steps_GEN pc_count p state1 mo = BER_Looping ll2) ==>
+    (bir_exec_steps_GEN pc_count p state0 (OPTION_MAP (\n2. n1+n2) mo) = BER_Looping
+         (LAPPEND (fromList l1) ll2))``,
+
+SIMP_TAC arith_ss [bir_exec_steps_GEN_EQ_Ended,
+  bir_exec_steps_GEN_EQ_Looping] >>
+REPEAT GEN_TAC >> REPEAT DISCH_TAC >>
+FULL_SIMP_TAC arith_ss [bir_exec_steps_observe_llist_NONE_ADD,
+  bir_exec_steps_observe_list_fromList,
+  bir_exec_infinite_steps_COUNT_STEPS_EQ_NONE, bir_exec_infinite_steps_fun_ADD] >>
+CONJ_TAC >- (
+  GEN_TAC >>
+  Cases_on `n < c_pc1` >- ASM_SIMP_TAC std_ss [] >>
+  METIS_TAC[arithmeticTheory.NOT_LESS, arithmeticTheory.LESS_EQ_EXISTS]
+) >>
+Cases_on `mo` >> FULL_SIMP_TAC std_ss [] >>
+REPEAT STRIP_TAC >>
+rename1 `bir_exec_infinite_steps_fun_COUNT_PCs _ _ _ i < n1 + n2` >>
+`n2 <> 0` by (
+  CCONTR_TAC >>
+  FULL_SIMP_TAC arith_ss []
+) >>
+Cases_on `i <= c_pc1` >- (
+  `bir_exec_infinite_steps_fun_COUNT_PCs pc_count p state0 i <= n1` by
+    METIS_TAC[bir_exec_infinite_steps_fun_COUNT_PCs_MONO,
+      arithmeticTheory.LESS_EQ_TRANS] >>
+  DECIDE_TAC
+) >>
+`c_pc1 <= i` by DECIDE_TAC >>
+`?i'. i = c_pc1 + i'` by METIS_TAC[arithmeticTheory.LESS_EQ_EXISTS] >>
+FULL_SIMP_TAC arith_ss [bir_exec_infinite_steps_fun_COUNT_PCs_ADD] >>
+Q.PAT_X_ASSUM `!i. _ < n2` (ASSUME_TAC o Q.SPEC `i'`) >>
+DECIDE_TAC);
+
+
+
+(***************************************************************)
+(* bir_exec_step_n                                             *)
+(***************************************************************)
+
+val bir_exec_step_n_TO_steps_GEN = store_thm ("bir_exec_step_n_TO_steps_GEN",
+  ``((bir_exec_step_n p state n = (l, c, state'))) <=>
+     (bir_exec_steps_GEN (\_. T) p state (SOME n) =
+     (BER_Ended l c c state'))``,
+
+`IS_BER_Ended (bir_exec_steps_GEN (\_. T) p state (SOME n))` by (
+  MATCH_MP_TAC bir_exec_steps_GEN_NOT_Looping_max_steps_blocks >>
+  SIMP_TAC std_ss []
+) >>
+FULL_SIMP_TAC (std_ss++bir_TYPES_ss++boolSimps.EQUIV_EXTRACT_ss) [
+  bir_exec_step_n_def, IS_BER_Ended_EXISTS,
+  valOf_BER_Ended_steps_def] >>
+FULL_SIMP_TAC std_ss [bir_exec_infinite_steps_fun_COUNT_PCs_EQ_COUNT_ALL_STEPS,
+  bir_exec_steps_GEN_EQ_Ended]);
+
 
 val bir_exec_step_n_EQ_THM = store_thm ("bir_exec_step_n_EQ_THM",
   ``((bir_exec_step_n p state n = (l, c, state'))) <=>
@@ -523,37 +1278,10 @@ val bir_exec_step_n_EQ_THM = store_thm ("bir_exec_step_n_EQ_THM",
         ~bir_state_is_terminated
            (bir_exec_infinite_steps_fun p state n)))``,
 
-`?l' c' st'. bir_exec_steps_opt p state (SOME n) = (l',SOME (c',st'))` by (
-  `~((SND (bir_exec_steps_opt p state (SOME n))) = NONE)` by (
-    SIMP_TAC std_ss [bir_exec_steps_opt_EQ_NONE_SND]
-  ) >>
-  Cases_on `bir_exec_steps_opt p state (SOME n)` >>
-  rename1 `_ = (l', xx)` >>
-  Cases_on `xx` >> FULL_SIMP_TAC std_ss [] >>
-  rename1 `_ = (l', SOME xx)` >>
-  Cases_on `xx` >>
-  SIMP_TAC std_ss []
-) >>
-
-ASM_SIMP_TAC std_ss [bir_exec_step_n_def, LET_THM] >>
-FULL_SIMP_TAC std_ss [bir_exec_steps_opt_EQ_SOME, bir_exec_steps_observe_llist_toList_SOME] >>
-REPEAT BasicProvers.VAR_EQ_TAC >>
-Cases_on `c = c'` >- (
-   ASM_SIMP_TAC (std_ss++boolSimps.EQUIV_EXTRACT_ss) [] >>
-   METIS_TAC[]
-) >>
-ASM_SIMP_TAC std_ss [] >>
-CCONTR_TAC >>
-Cases_on `~(bir_state_is_terminated state')` >- (
-  FULL_SIMP_TAC std_ss [] >>
-  `(c' < c) /\ (c = n)` by DECIDE_TAC >>
-  METIS_TAC[]
-) >>
-FULL_SIMP_TAC arith_ss [] >> REPEAT BasicProvers.VAR_EQ_TAC >>
-
-`~(c < c')` by METIS_TAC[] >>
-`(c' < c) /\ (c' < n)` by DECIDE_TAC >>
-METIS_TAC[]);
+SIMP_TAC std_ss [bir_exec_step_n_TO_steps_GEN] >>
+FULL_SIMP_TAC (arith_ss++boolSimps.EQUIV_EXTRACT_ss) [bir_exec_steps_GEN_EQ_Ended,
+  bir_exec_infinite_steps_fun_COUNT_PCs_EQ_COUNT_ALL_STEPS,
+  bir_state_COUNT_PC_ALL_STEPS]);
 
 
 val bir_exec_step_n_combine = store_thm ("bir_exec_step_n_combine",
@@ -562,23 +1290,10 @@ val bir_exec_step_n_combine = store_thm ("bir_exec_step_n_combine",
     (bir_exec_step_n p state1 n2 = (l2, c2, state2)) ==>
     (bir_exec_step_n p state0 (n1 + n2) = (l1++l2, c1+c2, state2))``,
 
-SIMP_TAC arith_ss [bir_exec_step_n_EQ_THM,
-  GSYM bir_exec_steps_observe_list_ADD,
-  bir_exec_infinite_steps_fun_ADD] >>
-REPEAT STRIP_TAC >- (
-  Cases_on `c1 < n1` >- (
-    FULL_SIMP_TAC bool_ss [GSYM bir_exec_infinite_steps_fun_ADD,
-      bir_exec_infinite_steps_fun_TERMINATED_0, combinTheory.K_DEF]
-  ) >>
-  `c1 = n1` by DECIDE_TAC >> BasicProvers.VAR_EQ_TAC >>
-  FULL_SIMP_TAC std_ss []
-) >- (
-  rename1 `n < _ + _` >>
-  Cases_on `n < c1` >- METIS_TAC [] >>
-  `?m. n = c1 + m` by METIS_TAC[arithmeticTheory.LESS_EQ_EXISTS, arithmeticTheory.NOT_LESS] >>
-  FULL_SIMP_TAC std_ss [] >>
-  METIS_TAC[]
-));
+REPEAT STRIP_TAC >>
+MP_TAC (Q.SPECL [`n1`, `SOME n2`] bir_exec_steps_GEN_SOME_ADD_Ended) >>
+FULL_SIMP_TAC std_ss [bir_exec_step_n_TO_steps_GEN] >>
+METIS_TAC[]);
 
 
 val bir_exec_step_n_add = store_thm ("bir_exec_step_n_add",
@@ -689,88 +1404,166 @@ SIMP_TAC (std_ss++boolSimps.EQUIV_EXTRACT_ss) [bir_exec_step_n_EQ_THM,
 
 
 (***************************************************************)
+(* bir_exec_block_n                                            *)
+(***************************************************************)
+
+val bir_exec_block_n_TO_steps_GEN = store_thm ("bir_exec_block_n_TO_steps_GEN",
+  ``((bir_exec_block_n p state n = (l, c_bl, c_st, state'))) <=>
+     (bir_exec_steps_GEN (\pc. pc.bpc_index = 0) p state (SOME n) =
+     (BER_Ended l c_bl c_st state'))``,
+
+`IS_BER_Ended (bir_exec_steps_GEN (\pc. pc.bpc_index = 0) p state (SOME n))` by (
+  MATCH_MP_TAC bir_exec_steps_GEN_NOT_Looping_max_steps_blocks >>
+  SIMP_TAC std_ss []
+) >>
+FULL_SIMP_TAC (std_ss++bir_TYPES_ss++boolSimps.EQUIV_EXTRACT_ss) [
+  bir_exec_block_n_def, IS_BER_Ended_EXISTS,
+  valOf_BER_Ended_def]);
+
+
+val bir_exec_block_n_EQ_THM = store_thm ("bir_exec_block_n_EQ_THM",
+  ``((bir_exec_block_n p state n = (l, c_st, c_bl, state'))) <=>
+
+    ((l = bir_exec_steps_observe_list p state c_st) /\
+     (c_bl = bir_exec_infinite_steps_fun_COUNT_PCs (\pc. pc.bpc_index = 0) p state c_st) /\
+     (c_bl <= n) /\ (c_bl < n ==> bir_state_is_terminated state') /\
+     (state' = bir_exec_infinite_steps_fun p state c_st) /\
+     ((bir_exec_infinite_steps_fun_COUNT_PCs (\pc. pc.bpc_index = 0) p state c_st = n) /\
+       0 < n ==>
+       (bir_state_COUNT_PC (\pc. pc.bpc_index = 0) (bir_exec_infinite_steps_fun p state c_st))) /\
+       (!n'. n' < c_st ==>
+          ~bir_state_is_terminated (bir_exec_infinite_steps_fun p state n') /\
+          bir_exec_infinite_steps_fun_COUNT_PCs (\pc. pc.bpc_index = 0) p state n' < n))``,
+
+SIMP_TAC (std_ss++boolSimps.EQUIV_EXTRACT_ss) [bir_exec_block_n_TO_steps_GEN,
+  bir_exec_steps_GEN_EQ_Ended, IMP_CONJ_THM, FORALL_AND_THM] >>
+REPEAT STRIP_TAC >>
+Tactical.REVERSE EQ_TAC >- (
+  REPEAT STRIP_TAC >>
+  Q.PAT_X_ASSUM `!n'. n' < c_st ==> _` (MP_TAC o Q.SPEC `n'`) >>
+  FULL_SIMP_TAC arith_ss []
+) >>
+REPEAT STRIP_TAC >>
+CCONTR_TAC >>
+FULL_SIMP_TAC arith_ss [arithmeticTheory.NOT_LESS] >>
+METIS_TAC[bir_exec_infinite_steps_fun_COUNT_PCs_COMPLETE_LESS_EQ,
+  arithmeticTheory.LESS_EQ_LESS_TRANS]);
+
+
+val bir_exec_block_n_combine = store_thm ("bir_exec_block_n_combine",
+  ``!p state0 state1 state2 n1 n2 l1 l2 c_bl1 c_bl2 c_st1 c_st2.
+    (bir_exec_block_n p state0 n1 = (l1, c_bl1, c_st1, state1)) ==>
+    (bir_exec_block_n p state1 n2 = (l2, c_bl2, c_st2, state2)) ==>
+    (bir_exec_block_n p state0 (n1 + n2) = (l1++l2, c_bl1+c_bl2, c_st1 + c_st2, state2))``,
+
+REPEAT STRIP_TAC >>
+MP_TAC (Q.SPECL [`n1`, `SOME n2`, `\pc. pc.bpc_index = 0`, `p`, `state0`]
+  bir_exec_steps_GEN_SOME_ADD_Ended) >>
+FULL_SIMP_TAC (std_ss++bir_TYPES_ss) [bir_exec_block_n_TO_steps_GEN]);
+
+
+val bir_exec_block_n_add = store_thm ("bir_exec_block_n_add",
+  ``!p state0 n1 n2.
+    (bir_exec_block_n p state0 (n1 + n2) =
+      let (l1, c_bl1, c_st1, state1) = bir_exec_block_n p state0 n1 in
+      let (l2, c_bl2, c_st2, state2) = bir_exec_block_n p state1 n2 in
+      (l1++l2, c_bl1+c_bl2, c_st1+c_st2, state2))``,
+
+REPEAT GEN_TAC >>
+`?l1 c_bl1 c_st1 state1. bir_exec_block_n p state0 n1 = (l1, c_bl1, c_st1, state1)` by METIS_TAC[pairTheory.PAIR] >>
+`?l2 c_bl2 c_st2 state2. bir_exec_block_n p state1 n2 = (l2, c_bl2, c_st2, state2)` by METIS_TAC[pairTheory.PAIR] >>
+ASM_SIMP_TAC std_ss [LET_THM] >>
+METIS_TAC[bir_exec_block_n_combine]);
+
+
+val bir_exec_block_n_REWR_0 = store_thm ("bir_exec_block_n_REWR_0",
+  ``!p state. bir_exec_block_n p state 0 = ([], 0, 0, state)``,
+SIMP_TAC std_ss [bir_exec_block_n_def, bir_exec_steps_GEN_REWR_no_steps,
+  valOf_BER_Ended_def]);
+
+
+val bir_exec_block_n_REWR_TERMINATED = store_thm ("bir_exec_block_n_REWR_TERMINATED",
+  ``!p state n. bir_state_is_terminated state ==> (bir_exec_block_n p state n = ([], 0, 0, state))``,
+SIMP_TAC std_ss [bir_exec_block_n_def, bir_exec_steps_GEN_REWR_TERMINATED,
+  valOf_BER_Ended_def]);
+
+
+(***************************************************************)
 (* bir_exec_steps                                              *)
 (***************************************************************)
 
-val bir_exec_steps_EQ_NONE = store_thm ("bir_exec_steps_EQ_NONE",
-  ``(bir_exec_steps p state = (ll, NONE)) <=>
+val bir_exec_steps_EQ_Looping = store_thm ("bir_exec_steps_EQ_Looping",
+  ``(bir_exec_steps p state = BER_Looping ll) <=>
     ((ll = bir_exec_steps_observe_llist p state NONE) /\
-     (bir_exec_infinite_steps_COUNT_STEPS p state = NONE))``,
+     (!n. ~bir_state_is_terminated (bir_exec_infinite_steps_fun p state n)))``,
 
-SIMP_TAC std_ss [bir_exec_steps_def, bir_exec_steps_opt_EQ_NONE]);
+SIMP_TAC std_ss [bir_exec_steps_def, bir_exec_steps_GEN_EQ_Looping,
+  bir_exec_infinite_steps_COUNT_STEPS_EQ_NONE]);
 
 
-val bir_exec_steps_EQ_SOME = store_thm ("bir_exec_steps_EQ_SOME",
-  ``((bir_exec_steps p state = (ll, SOME (c, state')))) <=>
-    ((ll = bir_exec_steps_observe_llist p state (SOME c)) /\
+val bir_exec_steps_EQ_Ended = store_thm ("bir_exec_steps_EQ_Ended",
+  ``((bir_exec_steps p state = BER_Ended l c1 c2 state') <=>
+    ((l = bir_exec_steps_observe_list p state c1) /\
+     (c1 = c2) /\
      bir_state_is_terminated state' /\
-     (state' = bir_exec_infinite_steps_fun p state c) /\
-     (!n. n < c ==> ~(bir_state_is_terminated (bir_exec_infinite_steps_fun p state n))))``,
+     (state' = bir_exec_infinite_steps_fun p state c1) /\
+     (!n. n < c1 ==> ~(bir_state_is_terminated (bir_exec_infinite_steps_fun p state n)))))``,
 
-SIMP_TAC std_ss [bir_exec_steps_def, bir_exec_steps_opt_EQ_SOME]);
+SIMP_TAC (std_ss++boolSimps.EQUIV_EXTRACT_ss) [bir_exec_steps_def, bir_exec_steps_GEN_EQ_Ended,
+  bir_exec_infinite_steps_fun_COUNT_PCs_EQ_COUNT_ALL_STEPS]);
 
 
 val bir_exec_steps_REWR_TERMINATED = store_thm ("bir_exec_steps_REWR_TERMINATED",
   ``bir_state_is_terminated state ==>
-    (bir_exec_steps p state = ([||], SOME (0, state)))``,
+    (bir_exec_steps p state = BER_Ended [] 0 0 state)``,
 
-SIMP_TAC std_ss [bir_exec_steps_def, bir_exec_steps_opt_REWR_TERMINATED]);
+SIMP_TAC std_ss [bir_exec_steps_def, bir_exec_steps_GEN_REWR_TERMINATED]);
 
 
 val bir_exec_steps_REWR_NOT_TERMINATED = store_thm ("bir_exec_steps_REWR_NOT_TERMINATED",
   ``~bir_state_is_terminated state ==>
     (bir_exec_steps p state =
        let (fe, state') = bir_exec_step p state in
-       let (ll,fst_opt) = bir_exec_steps p state' in
-       ((OPT_LCONS fe ll),
-        OPTION_MAP (\ (i,st). (SUC i, st)) fst_opt))``,
+       case bir_exec_steps p state' of
+         BER_Ended ol step_count pc_count st_final =>
+           BER_Ended (OPT_CONS fe ol) (SUC step_count) (SUC pc_count)
+             st_final
+         | BER_Looping oll => BER_Looping (OPT_LCONS fe oll))``,
 
-SIMP_TAC std_ss [bir_exec_steps_def, bir_exec_steps_opt_REWR_NOT_TERMINATED,
-  OPT_NUM_PRE_def, LET_THM]);
+SIMP_TAC std_ss [bir_exec_steps_def, bir_exec_steps_GEN_REWR_STEP,
+  OPT_NUM_PRE_def, LET_THM, bir_state_COUNT_PC_ALL_STEPS]);
 
 
 val bir_exec_steps_combine = store_thm ("bir_exec_steps_combine",
   ``!p state0 n1 state1 c1 l1.
     (bir_exec_step_n p state0 n1 = (l1, c1, state1)) ==>
     (bir_exec_steps p state0 =
-       (let (ll2, sto) = bir_exec_steps p state1 in
-        (LAPPEND (fromList l1) ll2, case sto of
-         | NONE => NONE
-         | SOME (c2, state2) => SOME (c1+c2, state2))))``,
+       case bir_exec_steps p state1 of
+         BER_Ended ol step_count pc_count st_final =>
+           BER_Ended (l1 ++ ol) (c1 + step_count) (c1 + pc_count)
+             st_final
+         | BER_Looping oll => BER_Looping (LAPPEND (fromList l1) oll))``,
 
 REPEAT STRIP_TAC >>
-`?ll2 sto. (bir_exec_steps p state1) = (ll2, sto)` by METIS_TAC[pairTheory.PAIR] >>
-FULL_SIMP_TAC std_ss [bir_exec_step_n_EQ_THM, LET_THM,
-  bir_exec_steps_observe_list_fromList] >>
-REPEAT BasicProvers.VAR_EQ_TAC >>
-Cases_on `sto` >- (
-  FULL_SIMP_TAC std_ss [bir_exec_steps_EQ_NONE, bir_exec_steps_observe_llist_NONE_ADD,
-    bir_exec_infinite_steps_COUNT_STEPS_EQ_NONE, bir_exec_infinite_steps_fun_ADD] >>
-  GEN_TAC >>
-  Cases_on `n < c1` >- METIS_TAC[] >>
-  METIS_TAC[arithmeticTheory.NOT_LESS, arithmeticTheory.LESS_EQ_EXISTS]
-) >- (
-  rename1 `_ = (_, SOME x)` >> Cases_on `x` >> rename1 `_ = (_, SOME (c2, state2))` >>
-  FULL_SIMP_TAC std_ss [bir_exec_steps_EQ_SOME, pairTheory.pair_case_thm,
-    bir_exec_steps_observe_llist_SOME_ADD, bir_exec_infinite_steps_fun_ADD] >>
-  REPEAT BasicProvers.VAR_EQ_TAC >> FULL_SIMP_TAC std_ss [] >>
-  GEN_TAC >>
-  Cases_on `n < c1` >- METIS_TAC[] >>
-  `?m. n = c1 + m` by METIS_TAC[arithmeticTheory.NOT_LESS, arithmeticTheory.LESS_EQ_EXISTS] >>
-  ASM_SIMP_TAC arith_ss []
-));
+MP_TAC (Q.SPECL [`n1`, `NONE`, `\_. T`, `p`, `state0`] bir_exec_steps_GEN_SOME_ADD_Ended) >>
+MP_TAC (Q.SPECL [`n1`, `NONE`, `\_. T`, `p`, `state0`] bir_exec_steps_GEN_SOME_ADD_Looping) >>
+FULL_SIMP_TAC (std_ss++bir_TYPES_ss) [bir_exec_step_n_TO_steps_GEN, GSYM bir_exec_steps_def] >>
 
+Cases_on `bir_exec_steps p state1` >> (
+  ASM_SIMP_TAC (std_ss++bir_TYPES_ss) []
+));
 
 
 val bir_exec_steps_combine_GUARD = store_thm ("bir_exec_steps_combine_GUARD",
   ``!p state0 n1 state1 c1 l1.
     (bir_exec_step_n p state0 n1 = (l1, c1, state1)) ==>
     (bir_exec_steps p state0 =
-       (if c1 < n1 then (fromList l1, SOME (c1, state1)) else (
-       (let (ll2, sto) = bir_exec_steps p state1 in
-       (LAPPEND (fromList l1) ll2), case sto of
-         | NONE => NONE
-         | SOME (c2, state2) => SOME (c1+c2, state2)))))``,
+       (if c1 < n1 then BER_Ended l1 c1 c1 state1 else (
+       case bir_exec_steps p state1 of
+         BER_Ended ol step_count pc_count st_final =>
+           BER_Ended (l1 ++ ol) (c1 + step_count) (c1 + pc_count)
+             st_final
+         | BER_Looping oll => BER_Looping (LAPPEND (fromList l1) oll))))``,
 
 REPEAT STRIP_TAC >>
 MP_TAC (Q.SPECL [`p`, `state0`, `n1`] bir_exec_steps_combine) >>
@@ -780,38 +1573,334 @@ Cases_on `c1 < n1` >> ASM_REWRITE_TAC[] >>
 `bir_state_is_terminated state1` by (
    FULL_SIMP_TAC std_ss [bir_exec_step_n_EQ_THM]
 ) >>
-FULL_SIMP_TAC std_ss [bir_exec_steps_REWR_TERMINATED, LET_THM,
-  LAPPEND_NIL_2ND, pairTheory.pair_case_thm]);
+FULL_SIMP_TAC (list_ss++bir_TYPES_ss) [bir_exec_steps_REWR_TERMINATED]);
 
 
 
 (***************************************************************)
-(* conversions to terminating executions                       *)
+(* conversions between various instances of bir_exec_steps_GEN *)
 (***************************************************************)
 
-(* If we terminate, we can use a finite number of steps to get exactly the same result *)
-val bir_exec_steps_opt_TO_bir_exec_step_n = store_thm ("bir_exec_steps_opt_TO_bir_exec_step_n",
-  ``!p st st' max_steps ll c.
-    (bir_exec_steps_opt p st max_steps = (ll, SOME (c, st'))) <=>
-    (?l. (bir_exec_step_n p st c = (l, c, st')) /\ (ll = fromList l) /\
-         (!m. (max_steps = SOME m) ==> c <= m) /\
-         ((!m. (max_steps = SOME m) ==> c < m) ==>
-         (bir_state_is_terminated st')))``,
+(* If we do not terminate, we can increase the max-step-count *)
+val bir_exec_steps_GEN_increase_max_steps_looping_SOME = store_thm (
+"bir_exec_steps_GEN_increase_max_steps_looping_SOME",
+  ``!pc_cond p st ll n1 n2.
+    (n1 <= n2) ==>
+    (bir_exec_steps_GEN pc_cond p st (SOME n1) = BER_Looping ll) ==>
+    (bir_exec_steps_GEN pc_cond p st (SOME n2) = BER_Looping ll)``,
 
-SIMP_TAC (std_ss++boolSimps.EQUIV_EXTRACT_ss) [bir_exec_steps_opt_EQ_SOME, bir_exec_step_n_EQ_THM,
-  bir_exec_steps_observe_list_fromList] >>
+SIMP_TAC arith_ss [bir_exec_steps_GEN_EQ_Looping,
+  bir_exec_infinite_steps_COUNT_STEPS_EQ_NONE] >>
 REPEAT STRIP_TAC >>
-Cases_on `max_steps` >> ASM_SIMP_TAC std_ss []);
+Q.PAT_X_ASSUM `!i. _` (MP_TAC o Q.SPEC `i`) >>
+ASM_SIMP_TAC arith_ss []);
 
 
+val bir_exec_steps_GEN_increase_max_steps_looping_NONE = store_thm (
+"bir_exec_steps_GEN_increase_max_steps_looping_NONE",
+  ``!pc_cond p st ll n.
+    (bir_exec_steps_GEN pc_cond p st (SOME n) = BER_Looping ll) ==>
+    (bir_exec_steps_GEN pc_cond p st NONE = BER_Looping ll)``,
+
+SIMP_TAC arith_ss [bir_exec_steps_GEN_EQ_Looping,
+  bir_exec_infinite_steps_COUNT_STEPS_EQ_NONE]);
+
+
+val bir_exec_steps_GEN_EQ_Ended_FIX_STEPS = store_thm (
+"bir_exec_steps_GEN_EQ_Ended_FIX_STEPS",
+  ``!pc_cond p st ol c_pc c_st st' mo.
+    ((bir_exec_steps_GEN pc_cond p st mo = BER_Ended ol c_st c_pc st')) ==>
+    (bir_exec_steps_GEN pc_cond p st (SOME
+       (if (bir_state_COUNT_PC pc_cond st' \/ (mo = SOME 0)) then c_pc else SUC c_pc)) = BER_Ended ol c_st c_pc st')``,
+
+REPEAT STRIP_TAC >>
+`(mo = SOME 0) ==> (c_st = 0)` by (
+  STRIP_TAC >>
+  FULL_SIMP_TAC (std_ss++bir_TYPES_ss) [bir_exec_steps_GEN_REWR_no_steps] >>
+  REPEAT (BasicProvers.VAR_EQ_TAC) >> REWRITE_TAC[]
+) >>
+FULL_SIMP_TAC std_ss [bir_exec_steps_GEN_EQ_Ended] >>
+REPEAT BasicProvers.VAR_EQ_TAC >>
+Q.ABBREV_TAC `cc =  bir_exec_infinite_steps_fun_COUNT_PCs pc_cond p st c_st` >>
+Q.ABBREV_TAC `st' = bir_exec_infinite_steps_fun p st c_st` >>
+
+Cases_on `bir_state_COUNT_PC pc_cond st'` >- (
+   FULL_SIMP_TAC std_ss [] >>
+   Q.UNABBREV_TAC `cc` >>
+   Q.UNABBREV_TAC `st'` >>
+   Cases_on `c_st` >- FULL_SIMP_TAC std_ss [] >>
+   FULL_SIMP_TAC std_ss [bir_exec_infinite_steps_fun_COUNT_PCs_END_DEF, LET_THM,
+     GSYM arithmeticTheory.LESS_EQ_IFF_LESS_SUC] >>
+   GEN_TAC >> STRIP_TAC >>
+   rename1 `(na:num) <= nb` >>
+   `bir_exec_infinite_steps_fun_COUNT_PCs pc_cond p st na <=
+    bir_exec_infinite_steps_fun_COUNT_PCs pc_cond p st nb` by
+    METIS_TAC[bir_exec_infinite_steps_fun_COUNT_PCs_MONO] >>
+   ASM_SIMP_TAC arith_ss []
+) >- (
+   Cases_on `mo = SOME 0` >- (
+     FULL_SIMP_TAC std_ss []
+   ) >>
+   CONJ_TAC >- (
+     Cases_on `mo` >> FULL_SIMP_TAC arith_ss []
+   ) >>
+   ASM_SIMP_TAC std_ss [] >>
+   REPEAT STRIP_TAC >>
+   `bir_exec_infinite_steps_fun_COUNT_PCs pc_cond p st n <= cc`
+      by METIS_TAC[bir_exec_infinite_steps_fun_COUNT_PCs_MONO,
+           arithmeticTheory.LESS_IMP_LESS_OR_EQ] >>
+   FULL_SIMP_TAC arith_ss []
+));
+
+
+val bir_exec_steps_GEN_increase_max_steps_Ended_NONE = store_thm (
+"bir_exec_steps_GEN_increase_max_steps_Ended_NONE",
+  ``!pc_cond p st ol c_pc c_st st' n.
+    (bir_state_is_terminated st') ==>
+    (bir_exec_steps_GEN pc_cond p st (SOME n) = BER_Ended ol c_pc c_st st') ==>
+    (bir_exec_steps_GEN pc_cond p st NONE = BER_Ended ol c_pc c_st st')``,
+
+SIMP_TAC std_ss [bir_exec_steps_GEN_EQ_Ended]);
+
+
+val bir_exec_steps_GEN_increase_max_steps_Ended_SOME = store_thm (
+"bir_exec_steps_GEN_increase_max_steps_Ended_SOME",
+  ``!pc_cond p st ol c_pc c_st st' n1 n2.
+    (n1 <= n2) ==>
+    (bir_state_is_terminated st') ==>
+    (bir_exec_steps_GEN pc_cond p st (SOME n1) = BER_Ended ol c_pc c_st st') ==>
+    (bir_exec_steps_GEN pc_cond p st (SOME n2) = BER_Ended ol c_pc c_st st')``,
+
+REPEAT STRIP_TAC >>
+`?i. n2 = n1 + i` by METIS_TAC[arithmeticTheory.LESS_EQ_EXISTS] >>
+FULL_SIMP_TAC std_ss [bir_exec_steps_GEN_EQ_Ended] >>
+Q.PAT_X_ASSUM `bir_state_is_terminated _` ASSUME_TAC >>
+REPEAT (BasicProvers.VAR_EQ_TAC) >>
+FULL_SIMP_TAC arith_ss [] >>
+REPEAT STRIP_TAC >>
+`n1 <= i + n1` by DECIDE_TAC >>
+METIS_TAC[bir_exec_infinite_steps_fun_COUNT_PCs_COMPLETE_LESS_EQ,
+      arithmeticTheory.LESS_EQ_LESS_TRANS]);
+
+
+
+val bir_exec_steps_GEN_change_cond_Looping_NONE = store_thm (
+"bir_exec_steps_GEN_change_cond_Looping_NONE",
+  ``!pc_cond pc_cond' mo p st ll.
+    (bir_exec_steps_GEN pc_cond p st mo = BER_Looping ll) ==>
+    (bir_exec_steps_GEN pc_cond' p st NONE = BER_Looping ll)``,
+
+SIMP_TAC std_ss [bir_exec_steps_GEN_EQ_Looping,
+  bir_exec_infinite_steps_COUNT_STEPS_EQ_NONE]);
+
+
+
+val bir_exec_steps_GEN_change_cond_Looping_SOME = store_thm (
+"bir_exec_steps_GEN_change_cond_Looping_SOME",
+  ``!pc_cond pc_cond' p st ll n1.
+    (!pc. pc_cond' pc ==> pc_cond pc) ==>
+    (bir_exec_steps_GEN pc_cond p st (SOME n1) = BER_Looping ll) ==>
+    (?n2. (n2 <= n1) /\ ((bir_exec_steps_GEN pc_cond' p st (SOME n2) = BER_Looping ll)))``,
+
+SIMP_TAC std_ss [bir_exec_steps_GEN_EQ_Looping,
+  bir_exec_infinite_steps_COUNT_STEPS_EQ_NONE,
+  GSYM FINITE_bir_exec_infinite_steps_fun_PC_COND_SET] >>
+REPEAT STRIP_TAC >>
+Q.EXISTS_TAC `SUC (CARD (bir_exec_infinite_steps_fun_PC_COND_SET pc_cond p st))` >>
+FULL_SIMP_TAC std_ss [GSYM arithmeticTheory.LESS_EQ,
+  GSYM arithmeticTheory.LESS_EQ_IFF_LESS_SUC] >>
+`(bir_exec_infinite_steps_fun_PC_COND_SET pc_cond' p st) SUBSET
+ (bir_exec_infinite_steps_fun_PC_COND_SET pc_cond p st)` suffices_by
+  METIS_TAC[SUBSET_FINITE, CARD_SUBSET] >>
+ASM_SIMP_TAC std_ss [SUBSET_DEF, IN_bir_exec_infinite_steps_fun_PC_COND_SET] >>
+METIS_TAC[bir_state_COUNT_PC_MONO]);
+
+
+
+val bir_exec_steps_GEN_change_cond_Ended_terminated = store_thm (
+"bir_exec_steps_GEN_change_cond_Ended_terminated",
+  ``!pc_cond pc_cond' p st ol c_pc c_st mo st'.
+    bir_state_is_terminated st' ==>
+    (bir_exec_steps_GEN pc_cond p st mo = BER_Ended ol c_st c_pc st') ==>
+    (?c_pc'. bir_exec_steps_GEN pc_cond' p st NONE = BER_Ended ol c_st c_pc' st')``,
+
+REPEAT STRIP_TAC >>
+FULL_SIMP_TAC std_ss [bir_exec_steps_GEN_EQ_Ended]);
+
+
+val bir_exec_steps_GEN_change_cond_Ended_NONE = store_thm (
+"bir_exec_steps_GEN_change_cond_Ended_NONE",
+  ``!pc_cond pc_cond' p st ol c_pc c_st st'.
+    (bir_exec_steps_GEN pc_cond p st NONE = BER_Ended ol c_st c_pc st') ==>
+    (?c_pc'. bir_exec_steps_GEN pc_cond' p st NONE = BER_Ended ol c_st c_pc' st')``,
+
+REPEAT STRIP_TAC >>
+FULL_SIMP_TAC std_ss [bir_exec_steps_GEN_EQ_Ended]);
+
+
+val bir_exec_steps_GEN_change_cond_Ended_SOME = store_thm (
+"bir_exec_steps_GEN_change_cond_Ended_SOME",
+  ``!pc_cond pc_cond' p st n1 ol c_pc c_st st'.
+    (!pc. pc_cond pc ==> pc_cond' pc) ==>
+    (bir_exec_steps_GEN pc_cond p st (SOME n1) = BER_Ended ol c_st c_pc st') ==>
+    ?n2 c_pc'. (n1 <= n2) /\ (bir_exec_steps_GEN pc_cond' p st (SOME n2) = BER_Ended ol c_st c_pc' st')``,
+
+REPEAT STRIP_TAC >>
+FULL_SIMP_TAC std_ss [bir_exec_steps_GEN_EQ_Ended]  >>
+REPEAT BasicProvers.VAR_EQ_TAC >>
+
+Q.ABBREV_TAC `cc = bir_exec_infinite_steps_fun_COUNT_PCs pc_cond' p st c_st` >>
+Q.ABBREV_TAC `st' = (bir_exec_infinite_steps_fun p st c_st)` >>
+`bir_exec_infinite_steps_fun_COUNT_PCs pc_cond p st c_st <= cc` by
+  METIS_TAC[bir_exec_infinite_steps_fun_COUNT_PCs_MONO_PC_COND] >>
+Cases_on `c_st` >- (
+  Q.UNABBREV_TAC `cc` >>
+  Q.EXISTS_TAC `n1` >>
+  FULL_SIMP_TAC arith_ss [bir_exec_infinite_steps_fun_COUNT_PCs_def]
+) >>
+rename1 `SUC c_st'` >>
+
+Cases_on `n1` >- (
+  Q.UNABBREV_TAC `cc` >>
+  Q.EXISTS_TAC `0` >>
+  Q.PAT_X_ASSUM `!n. n < _ ==> _` (MP_TAC o Q.SPEC `0`) >>
+  FULL_SIMP_TAC arith_ss [bir_exec_infinite_steps_fun_COUNT_PCs_def,
+    arithmeticTheory.NOT_LESS]
+) >>
+rename1 `SUC n1' <= _` >>
+
+Cases_on `n1' < cc` >- (
+  Cases_on `bir_state_COUNT_PC pc_cond' st'` >- (
+    Q.EXISTS_TAC `cc` >>
+    Q.UNABBREV_TAC `cc` >>
+    FULL_SIMP_TAC arith_ss [GSYM arithmeticTheory.LESS_EQ_IFF_LESS_SUC] >>
+    ASM_SIMP_TAC std_ss [bir_exec_infinite_steps_fun_COUNT_PCs_END_DEF, LET_THM] >>
+    REPEAT STRIP_TAC  >>
+    `bir_exec_infinite_steps_fun_COUNT_PCs pc_cond' p st n <=
+     bir_exec_infinite_steps_fun_COUNT_PCs pc_cond' p st c_st'` by
+       METIS_TAC [bir_exec_infinite_steps_fun_COUNT_PCs_MONO] >>
+    DECIDE_TAC
+  ) >- (
+    Q.EXISTS_TAC `SUC cc` >>
+    `~(bir_state_COUNT_PC pc_cond st')` by METIS_TAC[bir_state_COUNT_PC_MONO] >>
+    FULL_SIMP_TAC arith_ss [GSYM arithmeticTheory.LESS_EQ_IFF_LESS_SUC] >>
+    Q.UNABBREV_TAC `cc` >>
+    ASM_SIMP_TAC std_ss [bir_exec_infinite_steps_fun_COUNT_PCs_END_DEF, LET_THM] >>
+    REPEAT STRIP_TAC  >>
+    `bir_exec_infinite_steps_fun_COUNT_PCs pc_cond' p st n <=
+     bir_exec_infinite_steps_fun_COUNT_PCs pc_cond' p st c_st'` by
+       METIS_TAC [bir_exec_infinite_steps_fun_COUNT_PCs_MONO] >>
+    DECIDE_TAC
+  )
+) >- (
+  Q.EXISTS_TAC `SUC n1'` >>
+  FULL_SIMP_TAC arith_ss [GSYM arithmeticTheory.LESS_EQ_IFF_LESS_SUC] >>
+  Q.UNABBREV_TAC `cc` >>
+  REPEAT STRIP_TAC >>
+  `SUC n1' <=
+   bir_exec_infinite_steps_fun_COUNT_PCs pc_cond' p st (SUC c_st')` by
+       METIS_TAC [bir_exec_infinite_steps_fun_COUNT_PCs_MONO,
+                  arithmeticTheory.LESS_EQ_SUC_REFL,
+                  arithmeticTheory.LESS_EQ_TRANS] >>
+  DECIDE_TAC
+));
+
+
+
+
+(**************************************)
+(* conversions for concrete instances *)
+(**************************************)
+
+
+val bir_exec_steps_GEN_TO_bir_exec_step_n = store_thm ("bir_exec_steps_GEN_TO_bir_exec_step_n",
+  ``!p st st' mo c_st c_pc ol pc_cond.
+    (bir_exec_steps_GEN pc_cond p st mo = BER_Ended ol c_st c_pc st') ==>
+    (bir_exec_step_n p st c_st = (ol, c_st, st'))``,
+
+SIMP_TAC (std_ss++boolSimps.EQUIV_EXTRACT_ss) [bir_exec_steps_GEN_EQ_Ended, bir_exec_step_n_EQ_THM]);
 
 val bir_exec_steps_TO_bir_exec_step_n = store_thm ("bir_exec_steps_TO_bir_exec_step_n",
-  ``!p st st' ll c.
-    (bir_exec_steps p st = (ll, SOME (c, st'))) <=>
-    (?l. (bir_exec_step_n p st c = (l, c, st')) /\ (ll = fromList l) /\
-         (bir_state_is_terminated st'))``,
+  ``!p st st' ol c_st c_pc.
+    (bir_exec_steps p st = BER_Ended ol c_st c_pc st') <=>
+    ((bir_exec_step_n p st c_st = (ol, c_st, st')) /\ (c_pc = c_st) /\
+      (bir_state_is_terminated st'))``,
 
-SIMP_TAC std_ss [bir_exec_steps_def, bir_exec_steps_opt_TO_bir_exec_step_n]);
+SIMP_TAC (std_ss++boolSimps.EQUIV_EXTRACT_ss) [bir_exec_steps_EQ_Ended,
+  bir_exec_step_n_EQ_THM]);
+
+
+val bir_exec_block_n_TO_bir_exec_step_n = store_thm ("bir_exec_block_n_TO_bir_exec_step_n",
+  ``!p st st' ol c_st c_pc m.
+    (bir_exec_block_n p st m = (ol, c_st, c_pc, st')) ==>
+    (bir_exec_step_n p st c_st = (ol, c_st, st'))``,
+
+SIMP_TAC (std_ss++boolSimps.EQUIV_EXTRACT_ss) [bir_exec_block_n_EQ_THM,
+  bir_exec_step_n_EQ_THM]);
+
+
+val bir_exec_block_n_TO_bir_exec_to_labels_n = store_thm ("bir_exec_block_n_TO_bir_exec_to_labels_n",
+  ``(bir_exec_block_n p st m = (ol, c_st, c_pc, st')) <=>
+    (bir_exec_to_labels_n UNIV p st m = BER_Ended ol c_st c_pc st')``,
+
+SIMP_TAC std_ss [bir_exec_block_n_TO_steps_GEN,
+  bir_exec_to_labels_n_def, IN_UNIV]);
+
+
+val bir_exec_to_labels_n_UNIV_REWR = store_thm ("bir_exec_to_labels_n_UNIV_REWR",
+  ``bir_exec_to_labels_n UNIV p st m =
+    let (ol, c_st, c_pc, st') = bir_exec_block_n p st m in
+    BER_Ended ol c_st c_pc st'``,
+
+`?ol c_st c_pc st'. bir_exec_block_n p st m = (ol, c_st, c_pc, st')`
+   by METIS_TAC[pairTheory.PAIR] >>
+ASM_SIMP_TAC std_ss [LET_THM] >>
+FULL_SIMP_TAC std_ss [bir_exec_block_n_TO_bir_exec_to_labels_n]);
+
+
+val bir_exec_to_labels_n_change_labels = store_thm ("bir_exec_to_labels_n_change_labels",
+  ``!ls p st n ls' st' ol c_st c_l.
+    (ls SUBSET ls') ==>
+    (bir_exec_to_labels_n ls p st n = BER_Ended ol c_st c_l st') ==>
+    (?n' c_l'. (n <= n') /\
+               (bir_exec_to_labels_n ls' p st n' = BER_Ended ol c_st c_l' st'))``,
+
+SIMP_TAC std_ss [bir_exec_to_labels_n_def] >>
+REPEAT STRIP_TAC >>
+MP_TAC (Q.SPECL [`\pc. (pc.bpc_index = 0) /\ pc.bpc_label IN ls`,
+                 `\pc. (pc.bpc_index = 0) /\ pc.bpc_label IN ls'`,
+                 `p`, `st`, `n`] bir_exec_steps_GEN_change_cond_Ended_SOME) >>
+FULL_SIMP_TAC (std_ss++bir_TYPES_ss) [SUBSET_DEF]);
+
+
+val bir_exec_to_labels_n_TO_bir_exec_block_n = store_thm ("bir_exec_to_labels_n_TO_bir_exec_block_n",
+  ``!ls p st n st' ol c_st c_l .
+    (bir_exec_to_labels_n ls p st n = BER_Ended ol c_st c_l st') ==>
+    (?m c_l'. (n <= m) /\ (bir_exec_block_n p st m = (ol, c_st, c_l', st')))``,
+
+SIMP_TAC std_ss [bir_exec_block_n_TO_bir_exec_to_labels_n] >>
+REPEAT STRIP_TAC >>
+MP_TAC (Q.SPECL [`ls`, `p`, `st`, `n`, `UNIV`] bir_exec_to_labels_n_change_labels) >>
+ASM_SIMP_TAC (std_ss++bir_TYPES_ss) [SUBSET_UNIV]);
+
+
+val bir_exec_to_labels_n_TO_bir_exec_step_n = store_thm ("bir_exec_to_labels_n_TO_bir_exec_step_n",
+  ``!ls p st n st' ol c_st c_l .
+    (bir_exec_to_labels_n ls p st n = BER_Ended ol c_st c_l st') ==>
+    (bir_exec_step_n p st c_st = (ol, c_st, st'))``,
+
+SIMP_TAC std_ss [bir_exec_to_labels_n_def,
+  bir_exec_step_n_EQ_THM, bir_exec_steps_GEN_EQ_Ended])
+
+
+
+val bir_exec_to_labels_n_TO_bir_exec_steps = store_thm ("bir_exec_to_labels_n_TO_bir_exec_steps",
+  ``!ls p st n ll .
+    (bir_exec_to_labels_n ls p st n = BER_Looping ll) ==>
+    (bir_exec_steps p st = BER_Looping ll)``,
+
+SIMP_TAC std_ss [bir_exec_to_labels_n_def, bir_exec_steps_def] >>
+METIS_TAC[bir_exec_steps_GEN_change_cond_Looping_NONE]);
 
 
 val bir_exec_step_n_LIMIT_STEP_NO = store_thm ("bir_exec_step_n_LIMIT_STEP_NO",
@@ -819,8 +1908,8 @@ val bir_exec_step_n_LIMIT_STEP_NO = store_thm ("bir_exec_step_n_LIMIT_STEP_NO",
     (bir_exec_step_n p st n = (l, c, st')) ==>
     (bir_exec_step_n p st c = (l, c, st'))``,
 
-SIMP_TAC std_ss [bir_exec_step_n_EQ_THM] >>
-METIS_TAC[]);
+SIMP_TAC std_ss [bir_exec_step_n_EQ_THM]);
+
 
 
 val _ = export_theory();
